Create Swap and Church numerals examples, fix bugs in class hierarchy functions, fix some preconditions in the reduction relation.

sequential/coq/javalite.v
@@ -28,9 +28,9 @@ Definition Boolean := bool.
       C)
  *)
 Inductive T : Set :=
- | T_Bool : Boolean -> T
+ | T_Bool
  | T_Unit
- | T_Class : C -> T.
+ | T_Class: C -> T.
 
 (* (x this
       id)
@@ -115,14 +115,14 @@ Definition MethodMap     := HashMap.t Method.
 Inductive CL : Set :=
  | ClassDecl : C -> option CL -> FieldTypeMap -> MethodMap -> CL.
 
-(* (μ (CL ...))
+(* (Mu (CL ...))
  *)
 Definition Mu := HashMap.t CL.
 
 Inductive ProgramEntryPoint : Set :=
- | Entrypoint : C -> M -> ProgramEntryPoint.
+ | EntryPoint : C -> M -> ProgramEntryPoint.
 
-(* (P (μ (C m)))
+(* (P (mu (C m)))
  *)
 Inductive P : Set :=
  | Program: Mu -> ProgramEntryPoint -> P.
@@ -147,8 +147,8 @@ Inductive Hv : Set :=
  *)
 Definition H := HashMap.t Hv.
 
-(* (η mt
-      (η [x -> loc]))
+(* (eta mt
+      (eta [x -> loc]))
  *)
 Inductive Eta : Set :=
  | Eta_mt    : Eta
@@ -167,7 +167,7 @@ Inductive Eta : Set :=
       (if * e else e -> k)
       (var T x := * in e -> k)
       (begin * (e ...) -> k)
-      (pop \u03b7 k))
+      (pop eta k))
  *)
 Inductive Continuation : Set :=
  | K_Return               : Continuation
@@ -184,7 +184,7 @@ Inductive Continuation : Set :=
  | K_Seq                  : Expression -> Continuation -> Continuation
  | K_Pop                  : Eta -> Continuation -> Continuation.
 
-Inductive State : Set := 
+Inductive State : Set :=
  | StateCons : Mu -> H -> Eta -> Expression -> Continuation -> State.
 
 Inductive ThreadState : Set :=
@@ -268,7 +268,6 @@ Theorem T_eq_dec:
  forall (x y:T), {x=y} + {x <> y}.
 Proof.
  decide equality.
- apply bool_dec.
  apply C_eq_dec.
 Qed.
 
@@ -444,9 +443,9 @@ Fixpoint get_class_hierarchy_gas_CL_to_CLList (n:nat) (cl: option CL) (mu:Mu) : 
  | S n' => match cl with
            | None    => None
            | Some cl => match cl with
-                        | ClassDecl class superclass _ _ => 
+                        | ClassDecl class superclass _ _ =>
                                     match superclass with
-                                    | None    => Some nil
+                                    | None    => Some (cl::nil) (* Important! Do not return nil *)
                                     | Some cl => option_map (fun x => (x ++ (cl :: nil)))
                                                  (get_class_hierarchy_gas_CL_to_CLList n' (get_parent_of_CL_as_CL cl) mu)
                                     end
@@ -469,15 +468,23 @@ Definition get_reversed_class_hierarchy_CL_to_CLList (n:nat) (cl:CL) (mu:Mu) : C
 Definition class_list_from_class_to_field_locations_map (c2flm:ClassToFieldLocationsMap) : CList :=
  map (fun p => (get_C_from_id (fst p))) (HashMap.elements c2flm).
 
+(* Not Useful
 Definition class_list_from_object (object:HeapObject) : CList :=
  match object with
  | HeapObj c2flm => class_list_from_class_to_field_locations_map c2flm
  end.
+*)
 
 Definition classes_of_parents_and_self (c:C) (mu:Mu) : option CList :=
  match (convert_C_to_CL c mu) with
  | None    => Some (c :: nil)
  | Some cl => Some (convert_CLList_to_CList (get_class_hierarchy_CL_to_CLList (HashMap.cardinal mu) cl mu))
+ end.
+
+Definition class_decls_of_parents_and_self (c:C) (mu:Mu) : option CLList :=
+ match (convert_C_to_CL c mu) with
+ | None    => None
+ | Some cl => Some (get_class_hierarchy_CL_to_CLList (HashMap.cardinal mu) cl mu)
  end.
 
 Fixpoint hierarchical_field_lookup_from_list (f:F) (cllist:CLList) (c2flm:ClassToFieldLocationsMap) : option Location :=
@@ -491,7 +498,7 @@ Fixpoint hierarchical_field_lookup_from_list (f:F) (cllist:CLList) (c2flm:ClassT
                             end
               end
  end.
- 
+
 Definition hierarchical_field_lookup (f:F) (c:C) (c2flm:ClassToFieldLocationsMap) (mu:Mu) : option Location :=
  match (convert_C_to_CL c mu) with
  | None    => None
@@ -571,7 +578,7 @@ Definition h_extend (h:H) (loc:Location) (hv:Hv) : H := HashMap.add (location_to
 Definition alloc_and_write_this_and_args (h:H) (varlist:ValueList) : H :=
 .
    (* allocate locations for "this" and the arguments *)
-   (h_malloc_n h (S (length varlist)))        = (loc_o::loclist) 
+   (h_malloc_n h (S (length varlist)))        = (loc_o::loclist)
 *)
 
 Fixpoint h_extend_star (h:H) (loclist:LocationList) (varlist:list V) : option H :=
@@ -625,19 +632,12 @@ Definition create_location_value_list (flm:FieldLocationMap) (fvm:FieldValueMap)
 Definition create_hierarchical_location_value_list (hl:list FieldLocationMap) (dvs:list FieldValueMap) :=
  map (fun hl_dvs => create_location_value_list (fst hl_dvs) (snd hl_dvs)) (combine hl dvs).
 
-Check create_hierarchical_location_value_list.
-(*
-XXX
-Definition combine_list_of_lists (l:list (list (Location * V))) :=
- fold_left app l nil.
-*)
-
 Fixpoint h_extend_star_hierarchical_map (h:H) (hl:list FieldLocationMap) (dvs:list FieldValueMap) : option H :=
  match hl, dvs with
  | flm::t, fvm::t' => match create_location_value_list flm fvm with
                       | nil => h_extend_star_hierarchical_map h t t'
                       | (loc, v)::tl => let (loclist, vlist) := (split tl) in
-                                        match (h_extend_star h loclist vlist) with
+                                        match (h_extend_star (h_extend h loc (Hv_v v)) loclist vlist) with
                                         | None => None
                                         | Some h' => (h_extend_star_hierarchical_map h' t t')
                                         end
@@ -677,17 +677,16 @@ Definition get_field_list (cl:CL) : FieldTypeMap :=
 
 Definition method_lookup (m:M) (cl:CL) : option Method := HashMap.find m (get_method_list cl).
 
-Fixpoint get_class_with_virtual_method (m:M) (classlist:list (option CL)) : option CL :=
+Fixpoint get_class_with_virtual_method (m:M) (classlist:list CL) : option CL :=
  match classlist with
- | nil        => None
- | None::t    => None (* since classlist should be a hierarchy list *)
- | Some cl::t => match method_lookup m cl with
-                 | Some method => Some cl
-                 | None        => get_class_with_virtual_method m t
-                 end
+ | nil   => None
+ | cl::t => match method_lookup m cl with
+            | Some method => Some cl
+            | None        => get_class_with_virtual_method m t
+            end
  end.
 
-Fixpoint get_virtual_method (m:M) (classlist:list (option CL)) : option Method :=
+Fixpoint get_virtual_method (m:M) (classlist:list CL) : option Method :=
  match (get_class_with_virtual_method m classlist) with
  | None    => None
  | Some cl => method_lookup m cl
@@ -712,9 +711,9 @@ Definition get_hierarchical_type_map (hfm:list FieldTypeMap) : list FieldTypeMap
 
 Definition get_default_value (t:T) : V :=
  match t with
- | T_Class c => V_Pointer Null
+ | T_Class _ => V_Pointer Null
  | T_Unit    => V_Unit
- | T_Bool _  => V_Bool false
+ | T_Bool    => V_Bool false
  end.
 
 Fixpoint create_default_values_hash_map elems : HashMap.t V :=
@@ -736,10 +735,39 @@ Definition make_heap_pointer (loc:Location) (c:C) := (Hv_v (V_Pointer (Addr loc 
 Definition argument_list_to_XList (arglist:ArgumentList) : IdList :=
  map (fun vardec => get_variable_name vardec) arglist.
 
+Definition get_field_ids (ftm:FieldTypeMap) : list id :=
+ map (fun el => fst el) (HashMap.elements ftm).
+
+Definition create_field_location_pairs (ftm:FieldTypeMap)
+                                       (loclist:LocationList) : list (id * Location) :=
+ (combine (get_field_ids ftm) loclist).
+
+Fixpoint create_field_location_map (pairs: list(id * Location)) : FieldLocationMap :=
+ match pairs with
+ | nil => HashMap.empty Location
+ | (x, loc)::t => HashMap.add x loc (create_field_location_map t)
+ end.
+
+Fixpoint build_class_loc_lists_helper (arg:list (C * (FieldTypeMap * LocationList)))
+ : ClassToFieldLocationsMap :=
+ match arg with
+ | nil  => HashMap.empty FieldLocationMap
+ | ((SomeClass c), (ftm, loclist))::t => HashMap.add c
+                                         (create_field_location_map (create_field_location_pairs ftm loclist))
+                                         (build_class_loc_lists_helper t)
+ end.
+
 (* "New" helpers *)
 Definition build_class_loc_lists (hcl:CList)
                                  (hfl:list FieldTypeMap)
-                                 (hl:list LocationList) : ClassToFieldLocationsMap := HashMap.empty FieldLocationMap.
+                                 (hl:list LocationList) : ClassToFieldLocationsMap :=
+ if (beq_nat (length hfl) (length hl)) then
+     let fields_and_locations := (combine hfl hl) in
+       (if (beq_nat (length hcl) (length fields_and_locations)) then
+           build_class_loc_lists_helper (combine hcl fields_and_locations)
+        else HashMap.empty FieldLocationMap)
+ else
+     HashMap.empty FieldLocationMap.
 
 Definition get_required_heap_space (l:list nat) : nat := fold_left plus l 0.
 
@@ -759,6 +787,19 @@ Definition h_malloc_n_star (h:H) (l:list nat) : list LocationList :=
 
 Definition get_value_lengths (hfvm:list FieldValueMap) : list nat :=
  map (fun fvm => HashMap.cardinal fvm) hfvm.
+
+Definition inject (prog : P) : State :=
+ match prog with
+ | Program mu entrypoint =>
+    match entrypoint with
+    | EntryPoint c m => (StateCons mu (HashMap.empty Hv) Eta_mt (MethodInvocation (NewClass c) m nil) K_Return)
+    end
+ end.
+
+Definition inject_with_state (s:State) (m:M) : State :=
+ match s with
+ | StateCons mu h eta e k => (StateCons mu h eta (MethodInvocation e m nil) K_Return)
+ end.
 
 (* -------------------------------------------------------------------------- *)
 (* ------------------------- Expression Reductions -------------------------- *)
@@ -875,7 +916,7 @@ Inductive ExprReduces : State -> State -> Prop :=
                (StateCons mu h_0 eta (Expr_V v) k)
 
  (* ------------------------------------------------------------------------- *)
- (* Pop \u03b7 (close scope) *)
+ (* Pop eta (close scope) *)
 
  | ER_PopEta :
   forall (mu:Mu) (h:H) (eta eta_0:Eta) (v:V) (k:Continuation),
@@ -976,17 +1017,12 @@ Inductive ExprReduces : State -> State -> Prop :=
 
  | ER_MethodInvocationRaw :
   forall (mu:Mu) (h h_0 h_tmp:H) (eta eta_0:Eta) (e_m:Expression) (k:Continuation)
-         (m:M) (varlist:list V) (c c_0 c_p C_t:C) (loc loc_o:Location) (loclist:LocationList)
+         (m:M) (varlist:list V) (c C_t:C) (loc loc_o:Location) (loclist:LocationList)
          (methodvars:IdList) (obj1:HeapObject) (arglist:ArgumentList) (t:T)
-         (clist:CList) (classlist:list (option CL)) (CL_t:CL),
+         (classlist:CLList) (CL_t:CL),
    (h_lookup h loc)                 = Some (Hv_object obj1) ->
-   (class_list_from_object obj1)    = (c_0 :: c_p :: clist) ->
+   (class_decls_of_parents_and_self c mu)      = Some classlist ->
 
-   (*
-   Ignore C_0 which is always object and look up the method starting in C_p
-   Find the last M declaration before the zero or more trailing "error"s
-   *)
-   (convert_CList_to_CLList mu (c_p::clist))   = classlist ->
    (get_class_with_virtual_method m classlist) = Some CL_t ->
    (convert_CL_to_C CL_t)                      = C_t       ->
    (method_lookup m CL_t)                      = Some (AMethod m t arglist e_m) ->
@@ -1019,14 +1055,15 @@ Inductive ExprReduces : State -> State -> Prop :=
          (listofclassfieldloclists : ClassToFieldLocationsMap)
          (hierarchicalfieldlocmap  : list FieldLocationMap),
 
-   (classes_of_parents_and_self c mu)                     = Some classlist        ->
+   (classes_of_parents_and_self c mu)                     = Some classlist        -> (* Must be hierarchical *)
+   (beq_nat O (length classlist))                         = false                 -> (* XXX Check Redex Model for this case *)
    (get_fields_of_parents_and_self_C c mu)                = hierarchicalfieldlist ->
    (get_hierarchical_type_map hierarchicalfieldlist)      = hierarchicaltypelist  ->
    (get_hierarchical_default_values hierarchicaltypelist) = defaultvalues         ->
 
    (h_malloc_n_star h (get_value_lengths defaultvalues))  = hierarchicallocations ->
    (create_hierarchical_field_location_map hierarchicallocations defaultvalues)  = hierarchicalfieldlocmap  ->
-   (h_extend_star_hierarchical_map h hierarchicalfieldlocmap defaultvalues)      = Some h_0 ->
+   (h_extend_star_hierarchical_map h hierarchicalfieldlocmap defaultvalues)      = Some h_0 -> (* XXX Ensure h_0 != nil *)
 
    (h_malloc h_0)                                                                = loc_1  ->
    (build_class_loc_lists classlist hierarchicalfieldlist hierarchicallocations) = listofclassfieldloclists ->
@@ -1129,7 +1166,7 @@ Proof.
 
  (** (h_lookup h loc_0) must be (Hv_v v) *)
  dispatch_invalid_state_with_congruence.
- 
+
  (** (h_lookup h loc_0) must be (Hv_v v) *)
  dispatch_invalid_state_with_congruence.
 
@@ -1166,12 +1203,12 @@ Proof.
  left.
  exists (StateCons m h e e0 (K_EqualityRightOperand v c)).
  apply ER_Equals2.
- 
+
  (** K_EqualityRightOperand *)
  left.
  exists (StateCons m h e (convert_to_boolean_expr (V_equals v v0)) c).
  apply ER_Equals3.
- 
+
  (** K_Cast *)
  destruct v.
  destruct p as [loc|].
@@ -1329,6 +1366,9 @@ Proof.
  remember (h_malloc h_0) as loc_1.
  remember (build_class_loc_lists classlist hierarchicalfieldlist hierarchicallocations) as listofclassfieldloclists.
  remember (h_extend h_0 loc_1 (Hv_object (HeapObj listofclassfieldloclists))) as h_1.
+ remember (beq_nat O (length classlist)) as nonempty_classlist.
+ destruct nonempty_classlist.
+ dispatch_invalid_state_with_congruence.
 
  left.
  exists (StateCons m h_1 e (convert_pointer_to_expr (Addr loc_1 c)) c0).
@@ -1358,15 +1398,8 @@ Proof.
 
  dispatch_invalid_state_with_congruence.
 
- remember (class_list_from_object obj1) as clist.
- destruct clist.
-
- dispatch_invalid_state_with_congruence.
-
- destruct clist.
- dispatch_invalid_state_with_congruence.
-
- remember (convert_CList_to_CLList m0 (c2::clist)) as classlist.
+ remember (class_decls_of_parents_and_self c0 m0) as optionclasslist.
+ destruct optionclasslist as [classlist|].
  remember (get_class_with_virtual_method m classlist) as optionCL_t.
 
  destruct optionCL_t as [CL_t|].
@@ -1391,8 +1424,8 @@ Proof.
 
  left.
  exists (StateCons m0 h_0 eta_0 e0 (K_Pop e c)).
- apply (ER_MethodInvocationRaw m0 h h_0 h_tmp e eta_0 e0 c m l c0 c1 c2 C_t
-                               loc loc_o loclist methodvars obj1 a t clist
+ apply (ER_MethodInvocationRaw m0 h h_0 h_tmp e eta_0 e0 c m l c0 C_t
+                               loc loc_o loclist methodvars obj1 a t
                                classlist CL_t); try congruence.
 
  symmetry in HeqoptionAMethod.
@@ -1402,6 +1435,7 @@ Proof.
  rewrite <- H_same_method in HeqoptionAMethod.
  apply HeqoptionAMethod.
 
+ dispatch_invalid_state_with_congruence.
  dispatch_invalid_state_with_congruence.
  dispatch_invalid_state_with_congruence.
  dispatch_invalid_state_with_congruence.
@@ -1470,31 +1504,31 @@ Proof.
  clear - k. induction k; intros H; inversion H.
  eapply IHk. rewrite H1. exact H2.
 
- absurd (k = k); eauto. rewrite H8 at 1. 
+ absurd (k = k); eauto. rewrite H8 at 1.
  clear - k. induction k; eauto; intros H; inversion H.
  eapply IHk. rewrite H1. exact H2.
 
- absurd (k = k); eauto. rewrite H8 at 1. 
+ absurd (k = k); eauto. rewrite H8 at 1.
  clear - k. induction k; eauto; intros H; inversion H.
  eapply IHk. rewrite H1. exact H2.
 
- absurd (k = k); eauto. rewrite H8 at 1. 
+ absurd (k = k); eauto. rewrite H8 at 1.
  clear - k. induction k; eauto; intros H; inversion H.
  eapply IHk. rewrite H1. exact H2.
 
- absurd (k = k); eauto. rewrite H7 at 1. 
+ absurd (k = k); eauto. rewrite H7 at 1.
  clear - k. induction k; eauto; intros H; inversion H.
  eapply IHk. rewrite H1. rewrite H2. exact H3.
 
- absurd (k = k); eauto. rewrite H8 at 1. 
+ absurd (k = k); eauto. rewrite H8 at 1.
  clear - k. induction k; eauto; intros H; inversion H.
  eapply IHk. rewrite H1. exact H2.
 
- absurd (k = k); eauto. rewrite H8 at 1. 
+ absurd (k = k); eauto. rewrite H8 at 1.
  clear - k. induction k; eauto; intros H; inversion H.
  eapply IHk. rewrite H1. rewrite <- H1. exact H2.
 
- absurd (k = k); eauto. rewrite H8 at 1. 
+ absurd (k = k); eauto. rewrite H8 at 1.
  clear - k. induction k; eauto; intros H; inversion H.
  eapply IHk. rewrite H1. rewrite H2. exact H3.
 
@@ -1511,3 +1545,1407 @@ TODO:
 
 2. Create a program for converting S-Expressions to runnable ML Javalite expressions
 *)
+
+(* ========================================================================== *)
+(* The Church numerals example *)
+
+(* Note: There is a bug/syntax error in the generation of the last member of a sequence expression, VoidExp must not be included *)
+
+(* Classes *)
+Definition __class__LambdaTerm        := (P_of_succ_nat 1).
+Definition __class__Function          := (P_of_succ_nat 2).
+Definition __class__Abstraction       := (P_of_succ_nat 3).
+Definition __class__Application       := (P_of_succ_nat 4).
+Definition __class__SetIfNotZero      := (P_of_succ_nat 5).
+Definition __class__Variable          := (P_of_succ_nat 6).
+Definition __class__Church            := (P_of_succ_nat 7).
+Definition __class__ChurchTest        := (P_of_succ_nat 8).
+
+(* Fields *)
+Definition __field__Abstraction__t    := (P_of_succ_nat 10).
+Definition __field__Abstraction__f    := (P_of_succ_nat 11).
+Definition __field__Abstraction__x    := (P_of_succ_nat 12).
+
+Definition __field__Application__s    := (P_of_succ_nat 13).
+Definition __field__Application__t    := (P_of_succ_nat 14).
+
+Definition __field__SetIfNotZero__x   := (P_of_succ_nat 15).
+Definition __field__SetIfNotZero__y   := (P_of_succ_nat 16).
+Definition __field__SetIfNotZero__bam := (P_of_succ_nat 17).
+Definition __field__Variable__fix     := (P_of_succ_nat 18).
+
+Definition __field__Church__x         := (P_of_succ_nat 19).
+Definition __field__Church__f         := (P_of_succ_nat 20).
+Definition __field__Church__m         := (P_of_succ_nat 21).
+Definition __field__Church__n         := (P_of_succ_nat 22).
+Definition __field__Church__g         := (P_of_succ_nat 23).
+Definition __field__Church__h         := (P_of_succ_nat 24).
+Definition __field__Church__u         := (P_of_succ_nat 25).
+Definition __field__Church__zero      := (P_of_succ_nat 26).
+Definition __field__Church__one       := (P_of_succ_nat 27).
+Definition __field__Church__two       := (P_of_succ_nat 28).
+Definition __field__Church__plus      := (P_of_succ_nat 29).
+Definition __field__Church__succ      := (P_of_succ_nat 30).
+Definition __field__Church__mult      := (P_of_succ_nat 31).
+Definition __field__Church__exp       := (P_of_succ_nat 32).
+
+Definition __field__ChurchTest__instance := (P_of_succ_nat 33).
+Definition __field__ChurchTest__two   := (P_of_succ_nat 34).
+Definition __field__ChurchTest__three := (P_of_succ_nat 35).
+Definition __field__ChurchTest__five  := (P_of_succ_nat 36).
+Definition __field__ChurchTest__sinz  := (P_of_succ_nat 37).
+
+(* Methods *)
+(* XXX These methods should be defined in LambdaTerm (in the Redex model) since
+       we implement virtual methods
+*)
+Definition __method__LambdaTerm__ar        := (P_of_succ_nat 40).
+Definition __method__LambdaTerm__cas       := (P_of_succ_nat 41).
+Definition __method__LambdaTerm__eval      := (P_of_succ_nat 42).
+Definition __method__LambdaTerm__isAe      := (P_of_succ_nat 43).
+Definition __method__LambdaTerm__isFree    := (P_of_succ_nat 44).
+Definition __method__Function__eval        := (P_of_succ_nat 45).
+
+Definition __method__Abstraction__construct_x_t   := (P_of_succ_nat 50).
+Definition __method__Abstraction__construct_x_f   := (P_of_succ_nat 51).
+Definition __method__Abstraction__construct_x_t_f := (P_of_succ_nat 52).
+Definition __method__Abstraction__ar              := __method__LambdaTerm__ar.
+Definition __method__Abstraction__cas             := __method__LambdaTerm__cas.
+Definition __method__Abstraction__eval            := __method__LambdaTerm__eval.
+Definition __method__Abstraction__isAe            := __method__LambdaTerm__isAe.
+Definition __method__Abstraction__isFree          := __method__LambdaTerm__isFree.
+Definition __method__Abstraction__ar_abstraction  := (P_of_succ_nat 53).
+Definition __method__Abstraction__br              := (P_of_succ_nat 54).
+
+Definition __method__Application__construct       := (P_of_succ_nat 55).
+Definition __method__Application__ar              := __method__LambdaTerm__ar.
+Definition __method__Application__cas             := __method__LambdaTerm__cas.
+Definition __method__Application__eval            := __method__LambdaTerm__eval.
+Definition __method__Application__isAe            := __method__LambdaTerm__isAe.
+Definition __method__Application__isFree          := __method__LambdaTerm__isFree.
+
+Definition __method__SetIfNotZero__construct      := (P_of_succ_nat 56).
+Definition __method__SetIfNotZero__doEval         := (P_of_succ_nat 57).
+Definition __method__SetIfNotZero__eval           := __method__Function__eval.
+
+Definition __method__Variable__ar                 := __method__LambdaTerm__ar.
+Definition __method__Variable__cas                := __method__LambdaTerm__cas.
+Definition __method__Variable__isAe               := __method__LambdaTerm__isAe.
+Definition __method__Variable__isFree             := __method__LambdaTerm__isFree.
+Definition __method__Variable__eval               := __method__LambdaTerm__eval.
+
+Definition __method__Church__construct            := (P_of_succ_nat 60).
+Definition __method__Church__zero                 := (P_of_succ_nat 61).
+Definition __method__Church__one                  := (P_of_succ_nat 62).
+Definition __method__Church__plus                 := (P_of_succ_nat 63).
+Definition __method__Church__succ                 := (P_of_succ_nat 64).
+Definition __method__Church__mult                 := (P_of_succ_nat 65).
+Definition __method__Church__exp                  := (P_of_succ_nat 66).
+Definition __method__Church__pred                 := (P_of_succ_nat 67).
+Definition __method__Church__minus                := (P_of_succ_nat 68).
+
+Definition __method__ChurchTest__m                := (P_of_succ_nat 70).
+Definition __method__ChurchTest__n                := (P_of_succ_nat 71).
+Definition __method__ChurchTest__methodInvokeTest := (P_of_succ_nat 72).
+Definition __method__ChurchTest__construct        := (P_of_succ_nat 73).
+Definition __method__ChurchTest__testZeroJavalite := (P_of_succ_nat 74).
+Definition __method__ChurchTest__testNotZeroJavalite              := (P_of_succ_nat 75).
+Definition __method__ChurchTest__testJavaliteVariableEquivalence  := (P_of_succ_nat 76).
+Definition __method__ChurchTest__testJavaliteVariableEquivalence2 := (P_of_succ_nat 77).
+
+(* Arguments *)
+Definition __arg__Abstraction__construct_x_t__x   := (P_of_succ_nat 80).
+Definition __arg__Abstraction__construct_x_t__t   := (P_of_succ_nat 81).
+Definition __arg__Abstraction__construct_x_f__x   := (P_of_succ_nat 82).
+Definition __arg__Abstraction__construct_x_f__f   := (P_of_succ_nat 83).
+Definition __arg__Abstraction__construct_x_t_f__x := (P_of_succ_nat 84).
+Definition __arg__Abstraction__construct_x_t_f__t := (P_of_succ_nat 85).
+Definition __arg__Abstraction__construct_x_t_f__f := (P_of_succ_nat 86).
+Definition __arg__Abstraction__cas__x             := (P_of_succ_nat 87).
+Definition __arg__Abstraction__cas__r             := (P_of_succ_nat 88).
+Definition __arg__Abstraction__isFree__x          := (P_of_succ_nat 89).
+Definition __arg__Abstraction__br__s              := (P_of_succ_nat 90).
+Definition __arg__Abstraction__ar_abstraction__x  := (P_of_succ_nat 91).
+Definition __arg__Abstraction__ar__oldVar         := (P_of_succ_nat 92).
+Definition __arg__Abstraction__ar__newVar         := (P_of_succ_nat 93).
+Definition __arg__Abstraction__isAe__x            := (P_of_succ_nat 94).
+
+Definition __arg__Application__construct__s       := (P_of_succ_nat 95).
+Definition __arg__Application__construct__t       := (P_of_succ_nat 96).
+Definition __arg__Application__cas__x             := (P_of_succ_nat 97).
+Definition __arg__Application__cas__r             := (P_of_succ_nat 98).
+Definition __arg__Application__isFree__x          := (P_of_succ_nat 99).
+Definition __arg__Application__ar__oldVar         := (P_of_succ_nat 100).
+Definition __arg__Application__ar__newVar         := (P_of_succ_nat 101).
+Definition __arg__Application__isAe__x            := (P_of_succ_nat 102).
+
+Definition __arg__SetIfNotZero__doEval__c         := (P_of_succ_nat 103).
+
+Definition __arg__Variable__cas__x                := (P_of_succ_nat 104).
+Definition __arg__Variable__cas__r                := (P_of_succ_nat 105).
+Definition __arg__Variable__isFree__x             := (P_of_succ_nat 106).
+Definition __arg__Variable__ar__oldVar            := (P_of_succ_nat 107).
+Definition __arg__Variable__ar__newVar            := (P_of_succ_nat 108).
+Definition __arg__Variable__isAe__x               := (P_of_succ_nat 109).
+
+Definition __arg__Church__plus__m                 := (P_of_succ_nat 110).
+Definition __arg__Church__plus__n                 := (P_of_succ_nat 111).
+Definition __arg__Church__succ__n                 := (P_of_succ_nat 112).
+Definition __arg__Church__mult__m                 := (P_of_succ_nat 113).
+Definition __arg__Church__mult__n                 := (P_of_succ_nat 114).
+Definition __arg__Church__exp__m                  := (P_of_succ_nat 115).
+Definition __arg__Church__exp__n                  := (P_of_succ_nat 116).
+Definition __arg__Church__pred__n                 := (P_of_succ_nat 117).
+Definition __arg__Church__minus__m                := (P_of_succ_nat 118).
+Definition __arg__Church__minus__n                := (P_of_succ_nat 119).
+
+Definition __arg__ChurchTest__m__x                := (P_of_succ_nat 120).
+
+(* Locals *)
+Definition __local__Abstraction__cas__v             := (P_of_succ_nat 121).
+Definition __local__Abstraction__cas__y             := (P_of_succ_nat 122).
+Definition __local__Abstraction__cas__z             := (P_of_succ_nat 123).
+Definition __local__Abstraction__isFree__v          := (P_of_succ_nat 124).
+Definition __local__Abstraction__br__v              := (P_of_succ_nat 125).
+Definition __local__Abstraction__ar_abstraction__y  := (P_of_succ_nat 126).
+Definition __local__Abstraction__ar__v              := (P_of_succ_nat 127).
+Definition __local__Abstraction__ar__y              := (P_of_succ_nat 128).
+Definition __local__Abstraction__ar__z              := (P_of_succ_nat 129).
+Definition __local__Abstraction__isAe__v            := (P_of_succ_nat 130).
+Definition __local__Abstraction__isAe__a            := (P_of_succ_nat 131).
+
+Definition __local__Application__cas__lop           := (P_of_succ_nat 132).
+Definition __local__Application__cas__rop           := (P_of_succ_nat 133).
+Definition __local__Application__cas__v             := (P_of_succ_nat 134).
+Definition __local__Application__isFree__v          := (P_of_succ_nat 135).
+Definition __local__Application__isAe__v            := (P_of_succ_nat 136).
+Definition __local__Application__isAe__a            := (P_of_succ_nat 137).
+Definition __local__Application__eval__lop          := (P_of_succ_nat 138).
+Definition __local__Application__eval__rop          := (P_of_succ_nat 139).
+Definition __local__Application__eval__v            := (P_of_succ_nat 140).
+Definition __local__Application__eval__a            := (P_of_succ_nat 141).
+
+Definition __local__Variable__cas__v                := (P_of_succ_nat 142).
+Definition __local__Variable__isFree__v             := (P_of_succ_nat 143).
+Definition __local__Variable__ar__v                 := (P_of_succ_nat 144).
+
+Definition __local__ChurchTest__construct__v                        := (P_of_succ_nat 145).
+Definition __local__ChurchTest__testZeroJavalite__c                 := (P_of_succ_nat 146).
+Definition __local__ChurchTest__testZeroJavalite__s                 := (P_of_succ_nat 147).
+Definition __local__ChurchTest__testNotZeroJavalite__c              := (P_of_succ_nat 148).
+Definition __local__ChurchTest__testNotZeroJavalite__s              := (P_of_succ_nat 149).
+Definition __local__ChurchTest__testJavaliteVariableEquivalence__x  := (P_of_succ_nat 150).
+Definition __local__ChurchTest__testJavaliteVariableEquivalence__y  := (P_of_succ_nat 151).
+Definition __local__ChurchTest__testJavaliteVariableEquivalence2__x := (P_of_succ_nat 152).
+Definition __local__ChurchTest__testJavaliteVariableEquivalence2__y := (P_of_succ_nat 153).
+
+(* Artificial locals - created when converting method invocations to use ANF *)
+Definition __local__Abstraction__cas__arg2 := (P_of_succ_nat 154).
+Definition __local__Abstraction__cas__arg3 := (P_of_succ_nat 155).
+Definition __local__Abstraction__cas__arg4 := __local__Abstraction__cas__arg2.
+Definition __local__Abstraction__cas__arg5 := __local__Abstraction__cas__arg3.
+Definition __local__Abstraction__br__arg1 := (P_of_succ_nat 156).
+Definition __local__Abstraction__ar_abstraction__arg1 := (P_of_succ_nat 157).
+Definition __local__Abstraction__ar_abstraction__arg2 := (P_of_succ_nat 158).
+Definition __local__Abstraction__ar__arg1   := (P_of_succ_nat 159).
+Definition __local__Abstraction__ar__arg2   := (P_of_succ_nat 160).
+Definition __local__Abstraction__ar__arg3   := (P_of_succ_nat 161).
+Definition __local__Abstraction__isAe__arg1 := (P_of_succ_nat 162).
+Definition __local__Abstraction__isAe__arg2 := (P_of_succ_nat 163).
+Definition __local__Abstraction__isAe__arg3 := (P_of_succ_nat 164).
+
+Definition __local__Application__ar__t1   := (P_of_succ_nat 165).
+Definition __local__Application__ar__t2   := (P_of_succ_nat 166).
+Definition __local__Application__isAe__t1 := (P_of_succ_nat 167).
+Definition __local__Application__isAe__t2 := (P_of_succ_nat 168).
+
+Definition __local__ChurchTest__methodInvokeTest__arg   := (P_of_succ_nat 169).
+Definition __local__ChurchTest__testZeroJavalite__t1    := (P_of_succ_nat 170).
+Definition __local__ChurchTest__testNotZeroJavalite__t1 := (P_of_succ_nat 171).
+
+Definition __local__Church__construct__t1    := (P_of_succ_nat 172).
+Definition __local__Church__construct__t2    := (P_of_succ_nat 173).
+Definition __local__Church__construct__arg1  := (P_of_succ_nat 174).
+Definition __local__Church__construct__arg2  := (P_of_succ_nat 175).
+Definition __local__Church__construct__arg3  := (P_of_succ_nat 176).
+Definition __local__Church__construct__arg4  := (P_of_succ_nat 177).
+Definition __local__Church__construct__arg5  := (P_of_succ_nat 178).
+Definition __local__Church__construct__arg6  := (P_of_succ_nat 179).
+Definition __local__Church__construct__arg7  := (P_of_succ_nat 180).
+Definition __local__Church__construct__arg8  := (P_of_succ_nat 181).
+Definition __local__Church__construct__arg9  := (P_of_succ_nat 182).
+Definition __local__Church__construct__arg10 := (P_of_succ_nat 183).
+Definition __local__Church__construct__arg11 := (P_of_succ_nat 184).
+Definition __local__Church__construct__arg12 := (P_of_succ_nat 185).
+Definition __local__Church__construct__arg13 := (P_of_succ_nat 186).
+Definition __local__Church__construct__arg14 := (P_of_succ_nat 187).
+Definition __local__Church__construct__arg15 := (P_of_succ_nat 188).
+Definition __local__Church__construct__arg16 := (P_of_succ_nat 189).
+
+Definition __local__SetIfNotZero__doEval__t1   := (P_of_succ_nat 190).
+Definition __local__SetIfNotZero__doEval__t2   := (P_of_succ_nat 191).
+Definition __local__SetIfNotZero__doEval__t3   := (P_of_succ_nat 192).
+Definition __local__SetIfNotZero__doEval__arg1 := (P_of_succ_nat 193).
+Definition __local__SetIfNotZero__doEval__arg3 := (P_of_succ_nat 194).
+Definition __local__SetIfNotZero__doEval__arg4 := (P_of_succ_nat 195).
+
+(* Classes *)
+Definition C_Abstraction := (SomeClass __class__Abstraction).
+Definition C_Application := (SomeClass __class__Application).
+Definition C_Church      := (SomeClass __class__Church).
+Definition C_ChurchTest  := (SomeClass __class__ChurchTest).
+Definition C_Function    := (SomeClass __class__Function).
+Definition C_LambdaTerm  := (SomeClass __class__LambdaTerm).
+Definition C_SetIfNotZero:= (SomeClass __class__SetIfNotZero).
+Definition C_Variable    := (SomeClass __class__Variable).
+
+Definition METHOD_Abstraction__construct_x_t :=
+ (AMethod __method__Abstraction__construct_x_t
+          (T_Class C_Abstraction)
+          ((VarDec __arg__Abstraction__construct_x_t__x (T_Class C_Variable))::
+           (VarDec __arg__Abstraction__construct_x_t__t (T_Class C_LambdaTerm))::
+           nil)
+          (SeqExp (FieldAssign (This) __field__Abstraction__t (Expr_X (SomeId __arg__Abstraction__construct_x_t__t)))
+                  (SeqExp (FieldAssign (This) __field__Abstraction__x (Expr_X (SomeId __arg__Abstraction__construct_x_t__x)))
+                          (SeqExp (FieldAssign (This) __field__Abstraction__f (Expr_V (V_Pointer Null)))
+                                  (Expr_X (This)))))).
+
+Definition METHOD_Abstraction__construct_x_f :=
+ (AMethod __method__Abstraction__construct_x_f
+          (T_Class C_Abstraction)
+          ((VarDec __arg__Abstraction__construct_x_f__x (T_Class C_Variable))::
+           (VarDec __arg__Abstraction__construct_x_f__f (T_Class C_Function))::
+           nil)
+          (SeqExp (FieldAssign (This) __field__Abstraction__t (Expr_X (SomeId __arg__Abstraction__construct_x_f__x)))
+                  (SeqExp (FieldAssign (This) __field__Abstraction__x (Expr_X (SomeId __arg__Abstraction__construct_x_f__x)))
+                          (SeqExp (FieldAssign (This) __field__Abstraction__f (Expr_X (SomeId __arg__Abstraction__construct_x_f__f)))
+                                  (Expr_X (This)))))).
+
+Definition METHOD_Abstraction__construct_x_t_f :=
+ (AMethod __method__Abstraction__construct_x_t_f
+          (T_Class C_Abstraction)
+          ((VarDec __arg__Abstraction__construct_x_t_f__x (T_Class C_Variable))::
+           (VarDec __arg__Abstraction__construct_x_t_f__t (T_Class C_LambdaTerm))::
+           (VarDec __arg__Abstraction__construct_x_t_f__f (T_Class C_Function))::
+           nil)
+          (SeqExp (FieldAssign (This) __field__Abstraction__t (Expr_X (SomeId __arg__Abstraction__construct_x_t_f__t)))
+                  (SeqExp (FieldAssign (This) __field__Abstraction__x (Expr_X (SomeId __arg__Abstraction__construct_x_t_f__x)))
+                          (SeqExp (FieldAssign (This) __field__Abstraction__f (Expr_X (SomeId __arg__Abstraction__construct_x_t_f__f)))
+                                  (Expr_X (This)))))).
+
+Definition METHOD_Abstraction__cas :=
+ (AMethod __method__Abstraction__cas
+          (T_Class C_LambdaTerm)
+          ((VarDec __arg__Abstraction__cas__x (T_Class C_Variable))::
+           (VarDec __arg__Abstraction__cas__r (T_Class C_LambdaTerm))::
+           nil)
+          (VarDecExp (VarDec __local__Abstraction__cas__v (T_Class C_LambdaTerm)) (Expr_V (V_Pointer Null))
+           (VarDecExp (VarDec __local__Abstraction__cas__y (T_Class C_Variable)) (FieldRef (Expr_X (This)) __field__Abstraction__x)
+            (VarDecExp (VarDec __local__Abstraction__cas__z (T_Class C_Variable)) (Expr_V (V_Pointer Null))
+             (SeqExp (IfExpr (Equality (Expr_X (SomeId __arg__Abstraction__cas__x))
+                                       (Expr_X (SomeId __local__Abstraction__cas__y)))
+                             (VarAssign (SomeId __local__Abstraction__cas__v) (Expr_X (This)))
+(* which method are we invoking here? *)
+                             (IfExpr (Equality (MethodInvocation (Expr_X (SomeId __arg__Abstraction__cas__r))
+                                                                 __method__LambdaTerm__isFree
+                                                                 ((SomeId __local__Abstraction__cas__y)::nil))
+                                               (Expr_V (V_Bool false)))
+                                     (VarDecExp (VarDec __local__Abstraction__cas__arg2 (T_Class C_LambdaTerm))
+                                                (MethodInvocation (FieldRef (Expr_X (This)) __field__Abstraction__t)
+                                                                  __method__Abstraction__cas
+                                                                  ((SomeId __arg__Abstraction__cas__x)::(SomeId __arg__Abstraction__cas__r)::nil))
+                                                (VarDecExp (VarDec __local__Abstraction__cas__arg2 (T_Class C_Function))
+                                                           (FieldRef (Expr_X (This)) __field__Abstraction__f)
+                                                           (VarAssign (SomeId __local__Abstraction__cas__v)
+                                                                      (MethodInvocation (NewClass C_Abstraction)
+                                                                                        __method__Abstraction__construct_x_t_f
+                                                                                        ((SomeId __local__Abstraction__cas__y)::
+                                                                                         (SomeId __local__Abstraction__cas__arg2)::
+                                                                                         (SomeId __local__Abstraction__cas__arg3)::nil)))))
+                                     (SeqExp (VarAssign (SomeId __local__Abstraction__cas__z)
+                                                        (NewClass C_Variable))
+                                             (*(var LambdaTerm arg2 := (((this $ t) @ ar (y z)) @ cas (x r)) in
+                                                    (var Function arg3 := (this $ f) in
+                                                        (v := ((new Abstraction) @ construct-x-t-f (z arg2 arg3))))) *)
+                                             (VarDecExp (VarDec __local__Abstraction__cas__arg4 (T_Class C_LambdaTerm))
+                                                        (MethodInvocation (MethodInvocation (FieldRef (Expr_X (This)) __field__Abstraction__t)
+                                                                                            __method__LambdaTerm__ar
+                                                                                            ((SomeId __local__Abstraction__cas__y)::(SomeId __local__Abstraction__cas__z)::nil))
+                                                                          __method__LambdaTerm__cas
+                                                                          ((SomeId __arg__Abstraction__cas__x)::(SomeId __arg__Abstraction__cas__r)::nil))
+                                                        (VarDecExp (VarDec __local__Abstraction__cas__arg5 (T_Class C_Function))
+                                                                   (FieldRef (Expr_X (This)) __field__Abstraction__f)
+                                                                   (VarAssign (SomeId __local__Abstraction__cas__v)
+                                                                              (MethodInvocation (NewClass C_Abstraction)
+                                                                                                __method__Abstraction__construct_x_t_f
+                                                                                                ((SomeId __local__Abstraction__cas__z)::
+                                                                                                 (SomeId __local__Abstraction__cas__arg4)::
+                                                                                                 (SomeId __local__Abstraction__cas__arg5)::nil))))))))
+                     (Expr_X (SomeId __local__Abstraction__cas__v))))))).
+
+(*
+           (bool isFree ([Variable x])
+                 (var bool v := false in
+                      (begin
+                        (if ((x == (this $ x)) == false)
+                            (if (((this $ t) @ isFree (x)) == true)
+                                (v := true)
+                                else
+                                (v := false))
+                            else
+                            (v := false))
+                        v)))
+*)
+Definition METHOD_Abstraction__isFree :=
+ (AMethod __method__Abstraction__isFree
+          T_Bool
+          ((VarDec __arg__Abstraction__isFree__x (T_Class C_Variable))::nil)
+          (VarDecExp (VarDec __local__Abstraction__isFree__v T_Bool)
+                     (Expr_V (V_Bool false))
+                     (SeqExp (IfExpr (Equality (Equality (Expr_X (SomeId __arg__Abstraction__isFree__x))
+                                                         (FieldRef (Expr_X (This)) __field__Abstraction__x))
+                                               (Expr_V (V_Bool false)))
+                                     (IfExpr (Equality (MethodInvocation (FieldRef (Expr_X (This)) __field__Abstraction__t)
+                                                                         __method__LambdaTerm__isFree
+                                                                         ((SomeId __arg__Abstraction__isFree__x)::nil))
+                                                       (Expr_V (V_Bool true)))
+                                             (VarAssign (SomeId __local__Abstraction__isFree__v) (Expr_V (V_Bool true)))
+                                             (VarAssign (SomeId __local__Abstraction__isFree__v) (Expr_V (V_Bool false))))
+                                     (VarAssign (SomeId __local__Abstraction__isFree__v) (Expr_V (V_Bool false))))
+                             (Expr_X (SomeId __local__Abstraction__isFree__v))))).
+
+(* (LambdaTerm br([LambdaTerm s])
+                       (var LambdaTerm v := ((this $ t) @ cas ((this $ x) s)) in
+                            (begin
+                              (if (((this $ f) == null) == false)
+                                  ((this $ f) @ eval ())
+                                  else
+                                  unit)
+                              v)))
+*)
+
+Definition METHOD_Abstraction__br :=
+ (AMethod __method__Abstraction__br
+          (T_Class C_LambdaTerm)
+          ((VarDec __arg__Abstraction__br__s (T_Class C_LambdaTerm))::nil)
+          (VarDecExp (VarDec __local__Abstraction__br__arg1 (T_Class C_LambdaTerm))
+                     (FieldRef (Expr_X This) __field__Abstraction__x)
+                     (VarDecExp (VarDec __local__Abstraction__br__v (T_Class C_LambdaTerm))
+                                (MethodInvocation (FieldRef (Expr_X (This)) __field__Abstraction__t)
+                                                  __method__LambdaTerm__cas
+                                                  (nil))
+                                (SeqExp (IfExpr (Equality (Equality (FieldRef (Expr_X This) __field__Abstraction__f)
+                                                                    (Expr_V (V_Pointer Null)))
+                                                          (Expr_V (V_Bool false)))
+                                                (MethodInvocation (FieldRef (Expr_X (This)) __field__Abstraction__f)
+                                                                  __method__Function__eval
+                                                                  (nil))
+                                                (Expr_V (V_Unit)))
+                                        (Expr_X (SomeId __local__Abstraction__br__v)))))).
+
+(*
+(LambdaTerm ar-abstraction([Variable x])
+               (var Variable y := (this $ x) in
+                    (var arg1 := ((this $ t) @ ar(y x)) in
+                        (var arg2 := (this $ f) in
+                            ((new Abstraction) @ construct-x-t-f (x arg1 arg2))))))
+*)
+
+Definition METHOD_Abstraction__ar_abstraction :=
+ (AMethod __method__Abstraction__ar_abstraction
+          (T_Class C_LambdaTerm)
+          ((VarDec __arg__Abstraction__ar_abstraction__x (T_Class C_Variable))::nil)
+
+          (VarDecExp (VarDec __local__Abstraction__ar_abstraction__y (T_Class C_Variable))
+                     (FieldRef (Expr_X This) __field__Abstraction__x)
+                     (VarDecExp (VarDec __local__Abstraction__ar_abstraction__arg1 (T_Class C_LambdaTerm))
+                                (MethodInvocation (FieldRef (Expr_X This) __field__Abstraction__t)
+                                                  __method__LambdaTerm__ar
+                                                  ((SomeId __local__Abstraction__ar_abstraction__y)::
+                                                   (SomeId __arg__Abstraction__ar_abstraction__x)::nil))
+                                (VarDecExp (VarDec __local__Abstraction__ar_abstraction__arg2 (T_Class C_Function))
+                                           (FieldRef (Expr_X This) __field__Abstraction__f)
+                                           (MethodInvocation (NewClass C_Abstraction)
+                                                             __method__Abstraction__construct_x_t_f
+                                                             ((SomeId __arg__Abstraction__isFree__x)::nil)))))).
+
+(*
+(LambdaTerm ar([Variable oldVar] [Variable newVar])
+                         (var LambdaTerm v := null in
+                              (var Variable y := (this $ x) in
+                                   (var Variable z := null in
+                                        (begin
+                                          (if (y == oldVar)
+                                              (v := this)
+                                              else
+                                              (if (y == newVar)
+                                                  (begin
+                                                    (z := (new Variable))
+                                                    (v := ((this @ ar-abstraction (z)) @ ar (oldVar newVar))))
+                                                  else
+                                                  (var arg1 := (this $ x) in
+                                                    (var arg2 := ((this $ t) @ ar (oldVar newVar)) in
+                                                     (var arg3 := (this $ f) in
+                                                       (v := ((new Abstraction) @ construct-x-t-f (arg1 arg2 arg3))))))))
+                                        v)))))
+*)
+
+Definition METHOD_Abstraction__ar :=
+ (AMethod __method__Abstraction__ar
+          (T_Class C_LambdaTerm)
+          ((VarDec __arg__Abstraction__ar__oldVar (T_Class C_Variable))::
+           (VarDec __arg__Abstraction__ar__newVar (T_Class C_Variable))::nil)
+
+          (VarDecExp (VarDec __local__Abstraction__ar__v (T_Class C_LambdaTerm))
+                     (Expr_V (V_Pointer Null))
+                     (VarDecExp (VarDec __local__Abstraction__ar__y (T_Class C_Variable))
+                                (FieldRef (Expr_X (This)) __field__Abstraction__x)
+                                (VarDecExp (VarDec __local__Abstraction__ar__z (T_Class C_Variable))
+                                           (Expr_V (V_Pointer Null))
+                                           (SeqExp (IfExpr (Equality (Expr_X (SomeId __local__Abstraction__ar__y))
+                                                                     (Expr_X (SomeId __arg__Abstraction__ar__oldVar)))
+                                                           (VarAssign (SomeId __local__Abstraction__ar__v)
+                                                                      (Expr_X This))
+                                                           (IfExpr (Equality (Expr_X (SomeId __local__Abstraction__ar__y))
+                                                                             (Expr_X (SomeId __arg__Abstraction__ar__newVar)))
+                                                                   (SeqExp (VarAssign (SomeId __local__Abstraction__ar__z)
+                                                                                      (NewClass C_Variable))
+                                                                           (VarAssign (SomeId __local__Abstraction__ar__v)
+                                                                                      (MethodInvocation (MethodInvocation (Expr_X This) __method__Abstraction__ar_abstraction ((SomeId __local__Abstraction__ar__z)::nil))
+                                                                                                        __method__LambdaTerm__ar
+                                                                                                        ((SomeId __arg__Abstraction__ar__oldVar)::
+                                                                                                         (SomeId __arg__Abstraction__ar__newVar)::
+                                                                                                         nil))))
+                                                                   (VarDecExp (VarDec __local__Abstraction__ar__arg1 (T_Class C_Variable))
+                                                                                      (FieldRef (Expr_X This) __field__Abstraction__x)
+                                                                                      (VarDecExp (VarDec __local__Abstraction__ar__arg2 (T_Class C_LambdaTerm))
+                                                                                                 (MethodInvocation (FieldRef (Expr_X This) __field__Abstraction__t)
+                                                                                                                   __method__LambdaTerm__ar
+                                                                                                                   ((SomeId __arg__Abstraction__ar__oldVar)::
+                                                                                                                    (SomeId __arg__Abstraction__ar__newVar)::
+                                                                                                                    nil))
+                                                                                                 (VarDecExp (VarDec __local__Abstraction__ar__arg3 (T_Class C_Function))
+                                                                                                            (FieldRef (Expr_X This) __field__Abstraction__f)
+                                                                                                            (VarAssign (SomeId __local__Abstraction__ar__v)
+                                                                                                                       (MethodInvocation (NewClass C_Abstraction)
+                                                                                                                                         __method__Abstraction__construct_x_t_f
+                                                                                                                                         ((SomeId __local__Abstraction__ar__arg1)::
+                                                                                                                                          (SomeId __local__Abstraction__ar__arg2)::
+                                                                                                                                          (SomeId __local__Abstraction__ar__arg3)::nil))))))))
+                                                   (Expr_X (SomeId __local__Abstraction__br__v))))))).
+
+(*
+(bool isAe ([LambdaTerm x])
+                (var bool v := false in
+                     (var Abstraction a := null in
+                          (begin
+                            (if (x instanceof Abstraction)
+                                (begin
+                                  (a := (Abstraction x))
+                                  (var LambdaTerm arg1 := (a $ x) in
+                                    (if (((this $ x) @ isAe (arg1)) == false)
+                                      (var Variable arg2 := (this $ x) in
+                                      (a := (Abstraction (a @ ar-abstraction (arg2)))))
+                                      else
+                                      unit))
+                                  (var arg3 := (a $ t) in
+                                  (v := ((this $ t) @ isAe (arg3)))))
+                                else
+                                unit)
+                            v))))
+*)
+
+Definition METHOD_Abstraction__isAe :=
+ (AMethod __method__Abstraction__isAe
+          T_Bool
+          ((VarDec __arg__Abstraction__isAe__x (T_Class C_LambdaTerm))::nil)
+
+          (VarDecExp (VarDec __local__Abstraction__isAe__v T_Bool)
+                     (Expr_V (V_Bool false))
+                     (VarDecExp (VarDec __local__Abstraction__isAe__a (T_Class C_Abstraction))
+                                (Expr_V (V_Pointer Null))
+                                (SeqExp (IfExpr (InstanceOf (Expr_X (SomeId __arg__Abstraction__isAe__x)) C_Abstraction)
+                                                (SeqExp (VarAssign (SomeId __local__Abstraction__isAe__a)
+                                                                   (Cast C_Abstraction (Expr_X (SomeId __arg__Abstraction__isAe__x))))
+                                                        (SeqExp
+                                                                (* (var LambdaTerm arg1 := (a $ x) in
+                                                                                                    (if (((this $ x) @ isAe (arg1)) == false)
+                                                                                                      (var Variable arg2 := (this $ x) in
+                                                                                                      (a := (Abstraction (a @ ar-abstraction (arg2)))))
+                                                                                                      else
+                                                                                                      unit))
+                                                                *)
+                                                                  (VarDecExp (VarDec __local__Abstraction__isAe__arg1 (T_Class C_LambdaTerm))
+                                                                             (FieldRef (Expr_X (SomeId __local__Abstraction__isAe__a)) __field__Abstraction__x)
+                                                                             (IfExpr (Equality (MethodInvocation (FieldRef (Expr_X This) __field__Abstraction__x)
+                                                                                                                 __method__Variable__isAe
+                                                                                                                 ((SomeId __local__Abstraction__isAe__arg1)::nil))
+                                                                                               (Expr_V (V_Bool false)))
+                                                                                     (VarDecExp (VarDec __local__Abstraction__isAe__arg2 (T_Class C_Variable))
+                                                                                                (FieldRef (Expr_X This) __field__Abstraction__x)
+                                                                                                (VarAssign (SomeId __local__Abstraction__isAe__a)
+                                                                                                           (Cast C_Abstraction (MethodInvocation (Expr_X (SomeId __local__Abstraction__isAe__a))
+                                                                                                                                                 __method__Abstraction__ar_abstraction
+                                                                                                                                                 ((SomeId __local__Abstraction__isAe__arg2)::nil)))))
+                                                                                     (Expr_V V_Unit)))
+                                                                (*
+                                                                (var LambdaTerm arg3 := (a $ t) in
+                                                                     (v := ((this $ t) @ isAe (arg3))))
+                                                                *)
+                                                                  (VarDecExp (VarDec __local__Abstraction__isAe__arg3 (T_Class C_LambdaTerm))
+                                                                             (FieldRef (Expr_X (SomeId __local__Abstraction__isAe__a)) __field__Abstraction__t)
+                                                                             (VarAssign (SomeId __local__Abstraction__isAe__v)
+                                                                                        (MethodInvocation (FieldRef (Expr_X This) __field__Abstraction__t)
+                                                                                                          __method__LambdaTerm__isAe (nil))))))
+                                                 (Expr_V V_Unit))
+                                        (Expr_X (SomeId __local__Abstraction__isAe__v)))))).
+
+Definition METHOD_Abstraction__eval :=
+ (AMethod __method__Abstraction__eval
+          (T_Class C_LambdaTerm)
+          (nil)
+          (Expr_X (This))).
+
+(*
+(Application construct ([LambdaTerm t] [LambdaTerm s])
+                        (begin (this $ t := t )
+                               (this $ s := s)
+                               this))
+*)
+Definition METHOD_Application__construct :=
+ (AMethod __method__Application__construct
+          (T_Class C_Application)
+          ((VarDec __arg__Application__construct__t (T_Class C_LambdaTerm))::(VarDec __arg__Application__construct__s (T_Class C_LambdaTerm))::nil)
+
+          (SeqExp (FieldAssign (This) __field__Application__t (Expr_X (SomeId __arg__Application__construct__t)))
+                  (SeqExp (FieldAssign (This) __field__Application__s (Expr_X (SomeId __arg__Application__construct__s)))
+                          (Expr_X This)))).
+
+(*
+(LambdaTerm cas ([Variable x] [LambdaTerm r])
+                       (var LambdaTerm lop := null in
+                            (var LambdaTerm rop := null in
+                                 (var LambdaTerm v := null in
+                                      (begin
+                                        (lop := ((this $ t) @ cas (x r)))
+                                        (rop := ((this $ s) @ cas (x r)))
+                                        (v := ((new Application) @ construct (lop rop)))
+                                        v)))))
+*)
+Definition METHOD_Application__cas :=
+ (AMethod __method__Application__cas
+          (T_Class C_LambdaTerm)
+          ((VarDec __arg__Application__cas__x (T_Class C_Variable))::(VarDec __arg__Application__cas__r (T_Class C_LambdaTerm))::nil)
+
+          (VarDecExp (VarDec __local__Application__cas__lop (T_Class C_LambdaTerm))
+                     (Expr_V (V_Pointer Null))
+                     (VarDecExp (VarDec __local__Application__cas__rop (T_Class C_LambdaTerm))
+                                (Expr_V (V_Pointer Null))
+                                (VarDecExp (VarDec __local__Application__cas__v (T_Class C_LambdaTerm))
+                                           (Expr_V (V_Pointer Null))
+                                           (SeqExp (VarAssign (SomeId __local__Application__cas__lop)
+                                                              (MethodInvocation (FieldRef (Expr_X This) __field__Application__t)
+                                                                                __method__LambdaTerm__cas
+                                                                                ((SomeId __arg__Application__cas__x)::(SomeId __arg__Application__cas__r)::nil)))
+                                                   (SeqExp (VarAssign (SomeId __local__Application__cas__rop)
+                                                                      (MethodInvocation (FieldRef (Expr_X This) __field__Application__s)
+                                                                                         __method__LambdaTerm__cas
+                                                                                           ((SomeId __arg__Application__cas__x)::(SomeId __arg__Application__cas__r)::nil)))
+                                                           (SeqExp (VarAssign (SomeId __local__Application__cas__v)
+                                                                                (MethodInvocation (NewClass C_Application) __method__Application__construct
+                                                                                                    ((SomeId __local__Application__cas__lop)::(SomeId __local__Application__cas__rop)::nil)))
+                                                                    (Expr_X (SomeId __local__Application__cas__v))))))))).
+
+(*
+(bool isFree ([Variable x])
+                 (var bool v := ((this $ t) @ isFree(x)) in
+                      (begin
+                        (if ((this $ s) @ isFree(x))
+                            (v := true)
+                            else
+                            unit)
+                        v)))
+*)
+Definition METHOD_Application__isFree :=
+ (AMethod __method__Application__isFree
+          T_Bool
+          ((VarDec __arg__Application__isFree__x T_Bool)::nil)
+          (VarDecExp (VarDec __local__Application__isFree__v T_Bool)
+                     (MethodInvocation (FieldRef (Expr_X This) __field__Application__t) __method__LambdaTerm__isFree ((SomeId __arg__Application__isFree__x)::nil))
+                     (SeqExp (IfExpr (MethodInvocation (FieldRef (Expr_X This) __field__Application__s) __method__LambdaTerm__isFree ((SomeId __arg__Application__isFree__x)::nil))
+                                     (VarAssign (SomeId __local__Application__isFree__v) (Expr_V (V_Bool true)))
+                                     (Expr_V V_Unit))
+                             (Expr_X (SomeId __local__Application__isFree__v))))).
+
+(*
+(LambdaTerm ar ([Variable oldVar] [Variable newVar])
+  (var LambdaTerm t1 := ((this $ t) @ ar(oldVar newVar)) in
+    (var LambdaTerm t2 := ((this $ s) @ ar(oldVar newVar)) in
+           ((new Application) @ construct (t1 t2)))))
+*)
+
+Definition METHOD_Application__ar :=
+ (AMethod __method__Application__ar
+          (T_Class C_LambdaTerm)
+          ((VarDec __arg__Application__ar__oldVar (T_Class C_Variable))::(VarDec __arg__Application__ar__newVar (T_Class C_Variable))::nil)
+
+          (VarDecExp (VarDec __local__Application__ar__t1 (T_Class C_LambdaTerm))
+                     (MethodInvocation (FieldRef (Expr_X This) __field__Application__t) __method__LambdaTerm__ar
+                                       ((SomeId __arg__Application__ar__oldVar)::(SomeId __arg__Application__ar__newVar)::nil))
+                     (VarDecExp (VarDec __local__Application__ar__t2 (T_Class C_LambdaTerm))
+                                (MethodInvocation (FieldRef (Expr_X This) __field__Application__s) __method__LambdaTerm__ar
+                                                  ((SomeId __arg__Application__ar__oldVar)::(SomeId __arg__Application__ar__newVar)::nil))
+                                (MethodInvocation (NewClass C_Application) __method__Application__construct
+                                                  ((SomeId __local__Application__ar__t1)::(SomeId __local__Application__ar__t2)::nil))))).
+
+(*
+(bool isAe ([LambdaTerm x])
+                 (var bool v := false in
+                      (begin
+                        (if (x instanceof Application)
+                            (var Application a := (Application x) in
+                             (var LambdaTerm t1 := (a $ t) in
+                              (var LambdaTerm t2 := (a $ s) in
+                                 (v := (if ((this $ t) @ isAe (t1))
+                                           ((this $ s) @ isAe (t2))
+                                           else
+                                           false)))))
+                            else
+                            unit)
+                        v)))
+*)
+
+Definition METHOD_Application__isAe :=
+ (AMethod __method__Application__isAe
+          T_Bool ((VarDec __arg__Application__isAe__x (T_Class C_LambdaTerm))::nil)
+
+          (VarDecExp (VarDec __local__Application__isAe__v T_Bool)
+                     (Expr_V (V_Bool false))
+                     (SeqExp (IfExpr (InstanceOf (Expr_X (SomeId __arg__Application__isAe__x)) C_Application)
+                                      (VarDecExp (VarDec __local__Application__isAe__a (T_Class C_Application))
+                                                (Cast C_Application (Expr_X (SomeId __arg__Application__isAe__x)))
+                                                (VarDecExp (VarDec __local__Application__isAe__t1 (T_Class C_LambdaTerm))
+                                                           (FieldRef (Expr_X (SomeId __local__Application__isAe__a)) __field__Application__t)
+                                                           (VarDecExp (VarDec __local__Application__isAe__t2 (T_Class C_LambdaTerm))
+                                                                      (FieldRef (Expr_X (SomeId __local__Application__isAe__a)) __field__Application__s)
+                                                                      (VarAssign (SomeId __local__Application__isAe__v)
+                                                                                 (IfExpr (MethodInvocation (FieldRef (Expr_X This) __field__Application__t)
+                                                                                                           __method__LambdaTerm__isAe
+                                                                                                           ((SomeId __local__Application__isAe__t1)::nil))
+                                                                                         (MethodInvocation (FieldRef (Expr_X This) __field__Application__s)
+                                                                                                           __method__LambdaTerm__isAe
+                                                                                                           ((SomeId __local__Application__isAe__t2)::nil))
+                                                                                         (Expr_V (V_Bool false)))))))
+                                     (Expr_V V_Unit))
+                             (Expr_X (SomeId __local__Application__isAe__v))))).
+
+(*
+(LambdaTerm eval ()
+                       (var LambdaTerm lop := ((this $ t) @ eval ()) in
+                            (var LambdaTerm rop := ((this $ s) @ eval ()) in
+                                 (var LambdaTerm v := null in
+                                      (begin
+                                        (if (lop instanceof Abstraction)
+                                            (var Abstraction a := (Abstraction lop) in
+                                                 (v := ((a @ br (rop)) @ eval ())))
+                                            else
+                                            (v := ((new Application) @ construct (lop rop))))
+                                        v)))))
+*)
+
+Definition METHOD_Application__eval :=
+ (AMethod __method__Application__eval
+          (T_Class C_LambdaTerm) (nil)
+
+          (VarDecExp (VarDec __local__Application__eval__lop (T_Class C_LambdaTerm))
+                     (MethodInvocation (FieldRef (Expr_X This) __field__Application__t) __method__LambdaTerm__eval nil)
+                     (VarDecExp (VarDec __local__Application__eval__rop (T_Class C_LambdaTerm))
+                                (MethodInvocation (FieldRef (Expr_X This) __field__Application__s) __method__LambdaTerm__eval nil)
+                                (VarDecExp (VarDec __local__Application__eval__v (T_Class C_LambdaTerm))
+                                           (Expr_V (V_Pointer Null))
+                                           (SeqExp (IfExpr (InstanceOf (Expr_X (SomeId __local__Application__eval__lop)) C_Abstraction)
+                                                           (VarDecExp (VarDec __local__Application__eval__a (T_Class C_Abstraction))
+                                                                      (Cast C_Abstraction (Expr_X (SomeId __local__Application__eval__lop)))
+                                                                      (VarAssign (SomeId __local__Application__eval__v)
+                                                                                 (MethodInvocation (MethodInvocation (Expr_X (SomeId __local__Application__eval__a)) __method__Abstraction__br ((SomeId __local__Application__eval__rop)::nil))
+                                                                                                      __method__LambdaTerm__eval nil)))
+                                                            (VarAssign (SomeId __local__Application__eval__v)
+                                                                       (MethodInvocation (NewClass C_Application)
+                                                                                         __method__Application__construct
+                                                                                         ((SomeId __local__Application__eval__lop)::(SomeId __local__Application__eval__rop)::nil))))
+                                                   (Expr_X (SomeId __local__Application__eval__v))))))).
+
+
+
+(*
+(bool m ([bool x])
+      x)
+*)
+Definition METHOD_ChurchTest__m :=
+ (AMethod __method__ChurchTest__m
+          T_Bool ((VarDec __arg__ChurchTest__m__x T_Bool)::nil) (Expr_X (SomeId __arg__ChurchTest__m__x))).
+
+(*
+(bool n () true)
+*)
+Definition METHOD_ChurchTest__n :=
+ (AMethod __method__ChurchTest__n
+          T_Bool (nil) (Expr_V (V_Bool true))).
+
+(*
+(bool methodInvokeTest ()
+  (var bool arg :=(this @ n ()) in
+                 (this @ m (arg))))
+*)
+
+Definition METHOD_ChurchTest__methodInvokeTest :=
+ (AMethod __method__ChurchTest__methodInvokeTest
+          T_Bool (nil)
+          (VarDecExp (VarDec __local__ChurchTest__methodInvokeTest__arg T_Bool)
+                     (MethodInvocation (Expr_X This) __method__ChurchTest__n (nil))
+                     (MethodInvocation (Expr_X This) __method__ChurchTest__m ((SomeId __local__ChurchTest__methodInvokeTest__arg)::nil)))).
+
+(*
+ChurchTest construct ()
+                       (var Church v := ((new Church) @ construct ()) in
+                            (begin
+                              (this $ instance := v)
+                              (this $ sinz := ((new SetIfNotZero) @ construct ()))
+                              this)))
+*)
+Definition METHOD_ChurchTest__construct :=
+ (AMethod __method__ChurchTest__construct
+          (T_Class C_ChurchTest) (nil)
+
+          (VarDecExp (VarDec __local__ChurchTest__construct__v (T_Class C_Church))
+                     (MethodInvocation (NewClass C_Church) __method__Church__construct (nil))
+                     (SeqExp (FieldAssign This __field__ChurchTest__instance (Expr_X (SomeId __local__ChurchTest__construct__v)))
+                             (SeqExp (FieldAssign This __field__ChurchTest__sinz (MethodInvocation (NewClass C_SetIfNotZero) __method__SetIfNotZero__construct (nil)))
+                                     (Expr_X This))))).
+
+(*
+(bool testZeroJavalite ()
+                 (var Church c := (this $ instance) in
+                      (var SetIfNotZero s := (this $ sinz) in
+                           (begin
+                             (s $ bam := false)
+                             (var LambdaTerm t1 := (c @ zero ()) in
+                              (s @ doEval (t1)))
+                             (s $ bam)))))
+*)
+
+Definition METHOD_ChurchTest__testZeroJavalite :=
+ (AMethod __method__ChurchTest__testZeroJavalite
+          T_Bool (nil)
+
+          (VarDecExp (VarDec __local__ChurchTest__testZeroJavalite__c (T_Class C_Church))
+                     (FieldRef (Expr_X This) __field__ChurchTest__instance)
+                     (VarDecExp (VarDec __local__ChurchTest__testZeroJavalite__s (T_Class C_SetIfNotZero))
+                                (FieldRef (Expr_X This) __field__ChurchTest__sinz)
+                                (SeqExp (FieldAssign (SomeId __local__ChurchTest__testZeroJavalite__s) __field__SetIfNotZero__bam (Expr_V (V_Bool false)))
+                                        (SeqExp (VarDecExp (VarDec __local__ChurchTest__testZeroJavalite__t1 (T_Class C_LambdaTerm))
+                                                           (MethodInvocation (Expr_X (SomeId __local__ChurchTest__testZeroJavalite__c)) __method__Church__zero nil)
+                                                           (MethodInvocation (Expr_X (SomeId __local__ChurchTest__testZeroJavalite__s)) __method__SetIfNotZero__doEval ((SomeId __local__ChurchTest__testZeroJavalite__t1)::nil)))
+                                                (FieldRef (Expr_X (SomeId __local__ChurchTest__testZeroJavalite__s)) __field__SetIfNotZero__bam)))))).
+
+(*
+(bool testNotZeroJavalite ()
+                (var Church c := (this $ instance) in
+                      (var SetIfNotZero s := (this $ sinz) in
+                           (begin
+                             (s $ bam := false)
+                             (var LambdaTerm t1 := (c @ one ()) in
+                             (s @ doEval (t1)))
+                             (s $ bam)))))
+*)
+
+Definition METHOD_ChurchTest__testNotZeroJavalite :=
+ (AMethod __method__ChurchTest__testNotZeroJavalite
+          T_Bool (nil)
+
+          (VarDecExp (VarDec __local__ChurchTest__testNotZeroJavalite__c (T_Class C_Church))
+                     (FieldRef (Expr_X This) __field__ChurchTest__instance)
+                     (VarDecExp (VarDec __local__ChurchTest__testNotZeroJavalite__s (T_Class C_SetIfNotZero))
+                                (FieldRef (Expr_X This) __field__ChurchTest__sinz)
+                                (SeqExp (FieldAssign (SomeId __local__ChurchTest__testNotZeroJavalite__s) __field__SetIfNotZero__bam (Expr_V (V_Bool false)))
+                                        (SeqExp (VarDecExp (VarDec __local__ChurchTest__testNotZeroJavalite__t1 (T_Class C_LambdaTerm))
+                                                           (MethodInvocation (Expr_X (SomeId __local__ChurchTest__testNotZeroJavalite__c)) __method__Church__one nil)
+                                                           (MethodInvocation (Expr_X (SomeId __local__ChurchTest__testNotZeroJavalite__s)) __method__SetIfNotZero__doEval ((SomeId __local__ChurchTest__testNotZeroJavalite__t1)::nil)))
+                                                (FieldRef (Expr_X (SomeId __local__ChurchTest__testNotZeroJavalite__s)) __field__SetIfNotZero__bam)))))).
+
+(*
+(bool testJavaliteVariableEquivalence ()
+                  (var Variable x := (new Variable) in
+                       (var Variable y := (new Variable) in
+                            (x == y))))
+*)
+Definition METHOD_ChurchTest__testJavaliteVariableEquivalence :=
+ (AMethod __method__ChurchTest__testJavaliteVariableEquivalence
+          T_Bool (nil)
+          (VarDecExp (VarDec __local__ChurchTest__testJavaliteVariableEquivalence__x (T_Class C_Variable))
+                     (NewClass C_Variable)
+                     (VarDecExp (VarDec __local__ChurchTest__testJavaliteVariableEquivalence__y (T_Class C_Variable))
+                                (NewClass C_Variable)
+                                (Equality (Expr_X (SomeId __local__ChurchTest__testJavaliteVariableEquivalence__x)) (Expr_X (SomeId __local__ChurchTest__testJavaliteVariableEquivalence__x)))))).
+
+(*
+(bool testJavaliteVariableEquivalence2 ()
+                  (var SetIfNotZero x := (new SetIfNotZero) in
+                       (var SetIfNotZero y := (new SetIfNotZero) in
+                            (begin
+                              (x $ bam := true)
+                              (x == y)))))
+*)
+Definition METHOD_ChurchTest__testJavaliteVariableEquivalence2 :=
+ (AMethod __method__ChurchTest__testJavaliteVariableEquivalence2
+          T_Bool (nil)
+          (VarDecExp (VarDec __local__ChurchTest__testJavaliteVariableEquivalence__x (T_Class C_Variable))
+                     (NewClass C_Variable)
+                     (VarDecExp (VarDec __local__ChurchTest__testJavaliteVariableEquivalence__y (T_Class C_Variable))
+                                (NewClass C_Variable)
+                                (Equality (Expr_X (SomeId __local__ChurchTest__testJavaliteVariableEquivalence__x)) (Expr_X (SomeId __local__ChurchTest__testJavaliteVariableEquivalence__x)))))).
+
+
+
+(*
+(Church construct()
+                   (begin
+                     (this $ x := (new Variable))
+                     (this $ f := (new Variable))
+                     (this $ n := (new Variable))
+
+                     (* What types should t1 and t2 be? *)
+                     (var Variable arg1 := (this $ f) in
+                      (var Variable t1 := (this $ x) in
+                       (var LambdaTerm t2 := (this $ x) in
+                        (var LambdaTerm arg2 := ((new Abstraction) @ construct-x-t (t1 t2)) in
+                         (this $ zero := ((new Abstraction) @ construct-x-t (arg1 arg2)))))))
+
+                     (var Variable arg3 := (this $ n) in
+                      (var Variable arg5 := (this $ f) in
+                       (var Variable arg7 := (this $ x) in
+                        (var LambdaTerm arg9 := (this $ f) in
+                         (var LambdaTerm arg13 := (this $ n) in
+                          (var LambdaTerm arg14 := (this $ f) in
+                           (var LambdaTerm arg11 := ((new Application) @ construct (arg13 arg14)) in
+                            (var LambdaTerm arg12 := (this $ x) in
+                             (var LambdaTerm arg10 := ((new Application) @ construct (arg11 arg12)) in
+                              (var LambdaTerm arg8 := ((new Application) @ construct (arg9 arg10)) in
+                               (var Variable arg6 := ((new Abstraction) @ construct-x-t (arg7 arg8)) in
+                                (var LambdaTerm arg4 := ((new Abstraction) @ construct-x-t ( arg5 arg6)) in
+                                 (this $ succ := ((new Abstraction) @ construct-x-t (arg3 arg4)))))))))))))))
+
+                     (var LambdaTerm arg15 := (this $ succ) in
+                      (var LambdaTerm arg16 := (this $ zero) in
+                       (this $ one := ((new Application) @ construct (arg15 arg16)))))
+
+                     this
+                     ))
+*)
+
+Definition METHOD_Church__construct :=
+ (AMethod __method__Church__construct
+          (T_Class C_Church)
+          (nil)
+
+          (SeqExp (FieldAssign This __field__Church__x (NewClass C_Variable))
+                  (SeqExp (FieldAssign This __field__Church__f (NewClass C_Variable))
+                          (SeqExp (FieldAssign This __field__Church__n (NewClass C_Variable))
+                                  (SeqExp
+(*
+                     (var Variable arg1 := (this $ f) in
+                      (var Variable t1 := (this $ x) in
+                       (var LambdaTerm t2 := (this $ x) in
+                        (var LambdaTerm arg2 := ((new Abstraction) @ construct-x-t (t1 t2)) in
+                         (this $ zero := ((new Abstraction) @ construct-x-t (arg1 arg2)))))))
+*)
+(VarDecExp (VarDec __local__Church__construct__arg1 (T_Class C_Variable))
+           (FieldRef (Expr_X This) __field__Church__f)
+           (VarDecExp (VarDec __local__Church__construct__t1 (T_Class C_Variable))
+                      (FieldRef (Expr_X This) __field__Church__x)
+                      (VarDecExp (VarDec __local__Church__construct__t2 (T_Class C_LambdaTerm))
+                                 (FieldRef (Expr_X This) __field__Church__x)
+                                 (VarDecExp (VarDec __local__Church__construct__arg2 (T_Class C_LambdaTerm))
+                                            (MethodInvocation (NewClass C_Abstraction)
+                                                              __method__Abstraction__construct_x_t
+                                                              ((SomeId __local__Church__construct__t1)::(SomeId __local__Church__construct__t2)::nil))
+                                            (FieldAssign This __field__Church__zero
+                                                         (MethodInvocation (NewClass C_Abstraction)
+                                                                           __method__Abstraction__construct_x_t
+((SomeId __local__Church__construct__arg1)::(SomeId __local__Church__construct__arg2)::nil)))))))
+
+
+(*
+                    (var Variable arg3 := (this $ n) in
+                      (var Variable arg5 := (this $ f) in
+                       (var Variable arg7 := (this $ x) in
+                        (var LambdaTerm arg9 := (this $ f) in
+                         (var LambdaTerm arg13 := (this $ n) in
+                          (var LambdaTerm arg14 := (this $ f) in
+                           (var LambdaTerm arg11 := ((new Application) @ construct (arg13 arg14)) in
+                            (var LambdaTerm arg12 := (this $ x) in
+                             (var LambdaTerm arg10 := ((new Application) @ construct (arg11 arg12))
+                              (var LambdaTerm arg8 := ((new Application) @ construct (arg9 arg10)) in
+                               (var Variable arg6 := ((new Abstraction) @ construct-x-t (arg7 arg8))
+                                (var LambdaTerm arg4 := ((new Abstraction) @ construct-x-t ( arg5 arg6)) in
+                                 (this $ succ := ((new Abstraction) @ construct-x-t (arg3 arg4)))))))))))))))
+*)
+(SeqExp
+(VarDecExp (VarDec __local__Church__construct__arg3 (T_Class C_Variable))
+ (FieldRef (Expr_X This) __field__Church__n)
+ (VarDecExp (VarDec __local__Church__construct__arg5 (T_Class C_Variable))
+  (FieldRef (Expr_X This) __field__Church__f)
+  (VarDecExp (VarDec __local__Church__construct__arg7 (T_Class C_Variable))
+   (FieldRef (Expr_X This) __field__Church__x)
+   (VarDecExp (VarDec __local__Church__construct__arg9 (T_Class C_LambdaTerm))
+    (FieldRef (Expr_X This) __field__Church__f)
+    (VarDecExp (VarDec __local__Church__construct__arg13 (T_Class C_LambdaTerm))
+     (FieldRef (Expr_X This) __field__Church__n)
+     (VarDecExp (VarDec __local__Church__construct__arg14 (T_Class C_LambdaTerm))
+      (FieldRef (Expr_X This) __field__Church__f)
+      (VarDecExp (VarDec __local__Church__construct__arg11 (T_Class C_LambdaTerm))
+       (MethodInvocation (NewClass C_Application) __method__Application__construct
+                         ((SomeId __local__Church__construct__arg13)::(SomeId __local__Church__construct__arg14)::nil))
+         (VarDecExp (VarDec __local__Church__construct__arg12 (T_Class C_LambdaTerm))
+          (FieldRef (Expr_X This) __field__Church__x)
+           (VarDecExp (VarDec __local__Church__construct__arg10 (T_Class C_LambdaTerm))
+             (MethodInvocation (NewClass C_Application) __method__Application__construct
+                               ((SomeId __local__Church__construct__arg11)::(SomeId __local__Church__construct__arg12)::nil))
+             (VarDecExp (VarDec __local__Church__construct__arg8 (T_Class C_LambdaTerm))
+               (MethodInvocation (NewClass C_Application) __method__Application__construct
+                               ((SomeId __local__Church__construct__arg9)::(SomeId __local__Church__construct__arg10)::nil))
+             (VarDecExp (VarDec __local__Church__construct__arg6 (T_Class C_Variable))
+               (MethodInvocation (NewClass C_Abstraction) __method__Abstraction__construct_x_t
+                               ((SomeId __local__Church__construct__arg7)::(SomeId __local__Church__construct__arg8)::nil))
+               (VarDecExp (VarDec __local__Church__construct__arg4 (T_Class C_LambdaTerm))
+                 (MethodInvocation (NewClass C_Abstraction) __method__Abstraction__construct_x_t
+                                 ((SomeId __local__Church__construct__arg5)::(SomeId __local__Church__construct__arg6)::nil))
+                 (FieldAssign This __field__Church__succ
+                              (MethodInvocation (NewClass C_Abstraction) __method__Abstraction__construct_x_t
+                                 ((SomeId __local__Church__construct__arg3)::(SomeId __local__Church__construct__arg4)::nil)))))))))))))))
+
+(*
+ (var arg15 := (this $ succ) in
+  (var arg16 := (this $ zero) in
+   (this $ one := ((new Application) @ construct (arg15 arg16)))))
+this
+*)
+(SeqExp
+ (VarDecExp (VarDec __local__Church__construct__arg15 (T_Class C_LambdaTerm))
+  (FieldRef (Expr_X This) __field__Church__succ)
+   (VarDecExp (VarDec __local__Church__construct__arg16 (T_Class C_LambdaTerm))
+     (FieldRef (Expr_X This) __field__Church__zero)
+     (FieldAssign This __field__Church__one
+       (MethodInvocation (NewClass C_Application) __method__Application__construct
+                         ((SomeId __local__Church__construct__arg15)::(SomeId __local__Church__construct__arg16)::nil)))))
+ (Expr_X This)))))))).
+(*
+(Abstraction zero ()
+     (this $ zero))
+*)
+Definition METHOD_Church__zero :=
+ (AMethod __method__Church__zero
+          (T_Class C_Abstraction)
+          (nil)
+          (FieldRef (Expr_X This) __field__Church__zero)).
+
+(*
+(Abstraction one ()
+     (this $ one))
+*)
+Definition METHOD_Church__one :=
+ (AMethod __method__Church__one
+          (T_Class C_Abstraction)
+          (nil)
+          (FieldRef (Expr_X This) __field__Church__one)).
+
+
+(*
+((Function construct ()
+                     (begin
+                       (this $ x := (new Variable))
+                       (this $ y := (new Variable))
+                       (this $ bam := false)
+                       this))
+*)
+Definition METHOD_SetIfNotZero__construct :=
+ (AMethod __method__SetIfNotZero__construct
+          (T_Class C_Function)
+          (nil)
+
+          (SeqExp (FieldAssign (This) __field__SetIfNotZero__x (NewClass C_Variable))
+                  (SeqExp (FieldAssign (This) __field__SetIfNotZero__y (NewClass C_Variable))
+                          (SeqExp (FieldAssign (This) __field__SetIfNotZero__bam (Expr_V (V_Bool false)))
+                                  (Expr_X This))))).
+(*
+(unit eval ()
+                 (this $ bam := true))
+*)
+Definition METHOD_SetIfNotZero__eval :=
+ (AMethod __method__SetIfNotZero__eval
+          T_Unit
+          (nil)
+          (FieldAssign (This) __field__SetIfNotZero__bam (Expr_V (V_Bool true)))).
+
+(*
+(unit doEval ([LambdaTerm c])
+  (var Variable arg1 := (this $ x) in
+   (var LambdaTerm t1 := ((new Abstraction) @ construct-x-f (arg1 this)) in
+    (var LambdaTerm t2 := ((new Application) @ construct (c t1)) in
+     (var Variable arg3 := (this $ y) in
+      (var Variable arg4 := (this $ y) in
+       (var LambdaTerm t3 := ((new Abstraction) @ construct-x-t (arg3 arg4)) in
+         (((new Application) @ construct (t2 t3)) @ eval ()))))))))
+*)
+
+Definition METHOD_SetIfNotZero__doEval :=
+ (AMethod __method__SetIfNotZero__doEval
+          T_Unit ((VarDec __arg__SetIfNotZero__doEval__c (T_Class C_LambdaTerm))::nil)
+
+          (VarDecExp (VarDec __local__SetIfNotZero__doEval__arg1 (T_Class C_Variable))
+                     (FieldRef (Expr_X This) __field__SetIfNotZero__x)
+                     (VarDecExp (VarDec __local__SetIfNotZero__doEval__t1 (T_Class C_LambdaTerm))
+                                (MethodInvocation (NewClass C_Abstraction)
+                                                  __method__Abstraction__construct_x_f
+                                                  ((SomeId __local__SetIfNotZero__doEval__arg1)::
+                                                   This::nil))
+                                (VarDecExp (VarDec __local__SetIfNotZero__doEval__t2 (T_Class C_LambdaTerm))
+                                           (MethodInvocation (NewClass C_Application)
+                                                  __method__Application__construct
+                                                  ((SomeId __arg__SetIfNotZero__doEval__c)::
+                                                   (SomeId __local__SetIfNotZero__doEval__t1)::nil))
+                                            (VarDecExp (VarDec __local__SetIfNotZero__doEval__arg3 (T_Class C_Variable))
+                                                       (FieldRef (Expr_X This) __field__SetIfNotZero__y)
+                                                       (VarDecExp (VarDec __local__SetIfNotZero__doEval__arg4 (T_Class C_Variable))
+                                                                  (FieldRef (Expr_X This) __field__SetIfNotZero__y)
+                                                                  (VarDecExp (VarDec __local__SetIfNotZero__doEval__t3 (T_Class C_LambdaTerm))
+                                                                            (MethodInvocation (NewClass C_Abstraction)
+                                                                                                __method__Abstraction__construct_x_t
+                                                                                                ((SomeId __local__SetIfNotZero__doEval__arg3)::
+                                                                                                (SomeId __local__SetIfNotZero__doEval__arg4)::nil))
+                                                                            (MethodInvocation (NewClass C_Application)
+                                                                                            __method__Application__construct
+                                                                                            ((SomeId __local__SetIfNotZero__doEval__t2)::
+                                                                                             (SomeId __local__SetIfNotZero__doEval__t3)::nil))))))))).
+
+
+
+(*
+(LambdaTerm cas ([Variable x] [LambdaTerm r])
+                       (var Variable v := this in
+                            (begin
+                              (if (this == x)
+                                  (v := r)
+                                  else
+                                  unit)
+                              v)))
+*)
+Definition METHOD_Variable__cas :=
+ (AMethod __method__Variable__cas
+        (T_Class C_LambdaTerm)
+        ((VarDec __arg__Variable__cas__x (T_Class C_Variable))::(VarDec __arg__Variable__cas__r (T_Class C_LambdaTerm))::nil)
+
+        (VarDecExp (VarDec __local__Variable__cas__v (T_Class C_Variable))
+                   (Expr_X This)
+                   (SeqExp (IfExpr (Equality (Expr_X This) (Expr_X (SomeId __arg__Variable__cas__x)))
+                                   (VarAssign (SomeId __local__Variable__cas__v) (Expr_X (SomeId __arg__Variable__cas__r)))
+                                   (Expr_V (V_Unit)))
+                           (Expr_X (SomeId __local__Variable__cas__v))))).
+
+(*
+(bool isFree ([Variable x])
+                 (var bool v := false in
+                      (begin
+                        (if (x == this)
+                            (v := true)
+                            else
+                            unit)
+                        v)))
+*)
+Definition METHOD_Variable__isFree :=
+ (AMethod __method__Variable__isFree
+        T_Bool
+        ((VarDec __arg__Variable__isFree__x (T_Class C_Variable))::nil)
+
+        (VarDecExp (VarDec __local__Variable__isFree__v T_Bool)
+                   (Expr_V (V_Bool false))
+                   (SeqExp (IfExpr (Equality (Expr_X (SomeId __arg__Variable__isFree__x)) (Expr_X This))
+                                   (VarAssign (SomeId __local__Variable__isFree__v) (Expr_V (V_Bool true)))
+                                   (Expr_V V_Unit))
+                           (Expr_X (SomeId __local__Variable__isFree__v))))).
+
+(*
+(LambdaTerm ar ([Variable oldVar] [Variable newVar])
+                       (var LambdaTerm v := this in
+                            (begin
+                              (if (oldVar == this)
+                                  (v := newVar)
+                                  else
+                                  unit)
+                              v)))
+*)
+Definition METHOD_Variable__ar :=
+ (AMethod __method__Variable__ar
+          (T_Class C_LambdaTerm)
+          ((VarDec __arg__Variable__ar__oldVar (T_Class C_Variable))::(VarDec __arg__Variable__ar__newVar (T_Class C_Variable))::nil)
+
+          (VarDecExp (VarDec __local__Variable__ar__v (T_Class C_LambdaTerm))
+                     (Expr_X (This))
+                     (SeqExp (IfExpr (Equality (Expr_X (SomeId __arg__Variable__ar__oldVar)) (Expr_X This))
+                                     (VarAssign (SomeId __local__Variable__ar__v) (Expr_X (SomeId __arg__Variable__ar__newVar)))
+                                     (Expr_V V_Unit))
+                             (Expr_X (SomeId __local__Variable__ar__v))))).
+
+(*
+(bool isAe ([LambdaTerm x])
+                 (x == this))
+*)
+Definition METHOD_Variable__isAe :=
+ (AMethod __method__Variable__isAe
+          T_Bool
+          ((VarDec __arg__Variable__isAe__x (T_Class C_LambdaTerm)::nil))
+          (Equality (Expr_X (SomeId __arg__Variable__isAe__x)) (Expr_X This))).
+
+(*
+(LambdaTerm eval ()
+        this)
+*)
+Definition METHOD_Variable__eval :=
+ (AMethod __method__Variable__eval
+          (T_Class C_LambdaTerm) (nil) (Expr_X This)).
+
+Definition CLASS_Object : option CL := None.
+
+
+Definition CLASS_Function :=
+ (ClassDecl C_Function CLASS_Object (HashMap.empty T) (HashMap.empty Method)).
+
+
+Definition CLASS_LambdaTerm :=
+ (ClassDecl C_LambdaTerm CLASS_Object (HashMap.empty T) (HashMap.empty Method)).
+
+Definition CLASS_Abstraction :=
+ (ClassDecl C_Abstraction (Some CLASS_LambdaTerm)
+            (HashMap.add __field__Abstraction__t (T_Class C_LambdaTerm)
+             (HashMap.add __field__Abstraction__x (T_Class C_Variable)
+             (HashMap.add __field__Abstraction__f (T_Class C_Function)
+             (HashMap.empty T))))
+            (HashMap.add  __method__Abstraction__construct_x_t   METHOD_Abstraction__construct_x_t
+             (HashMap.add __method__Abstraction__construct_x_f   METHOD_Abstraction__construct_x_f
+             (HashMap.add __method__Abstraction__construct_x_t_f METHOD_Abstraction__construct_x_t_f
+             (HashMap.add __method__Abstraction__cas             METHOD_Abstraction__cas
+             (HashMap.add __method__Abstraction__isFree          METHOD_Abstraction__isFree
+             (HashMap.add __method__Abstraction__br              METHOD_Abstraction__br
+             (HashMap.add __method__Abstraction__ar_abstraction  METHOD_Abstraction__ar_abstraction
+             (HashMap.add __method__Abstraction__ar              METHOD_Abstraction__ar
+             (HashMap.add __method__Abstraction__isAe            METHOD_Abstraction__isAe
+             (HashMap.add __method__Abstraction__eval            METHOD_Abstraction__eval
+             (HashMap.empty Method)))))))))))).
+
+Definition CLASS_Application :=
+ (ClassDecl C_Application (Some CLASS_LambdaTerm)
+            (HashMap.add __field__Application__s (T_Class C_LambdaTerm)
+             (HashMap.add __field__Application__t (T_Class C_LambdaTerm)
+             (HashMap.empty T)))
+            (HashMap.add  __method__Application__construct METHOD_Application__construct
+             (HashMap.add __method__Application__cas       METHOD_Application__cas
+             (HashMap.add __method__Application__isFree    METHOD_Application__isFree
+             (HashMap.add __method__Application__ar        METHOD_Application__ar
+             (HashMap.add __method__Application__isAe      METHOD_Application__isAe
+             (HashMap.add __method__Application__eval      METHOD_Application__eval
+             (HashMap.empty Method)))))))).
+
+Definition CLASS_ChurchTest :=
+ (ClassDecl C_ChurchTest CLASS_Object
+            (HashMap.add __field__ChurchTest__instance (T_Class C_Church)
+             (HashMap.add __field__ChurchTest__two   (T_Class C_LambdaTerm)
+             (HashMap.add __field__ChurchTest__three (T_Class C_LambdaTerm)
+             (HashMap.add __field__ChurchTest__five  (T_Class C_LambdaTerm)
+             (HashMap.add __field__ChurchTest__sinz  (T_Class C_SetIfNotZero)
+             (HashMap.empty T))))))
+            (HashMap.add  __method__ChurchTest__m                                METHOD_ChurchTest__m
+             (HashMap.add  __method__ChurchTest__n                               METHOD_ChurchTest__n
+             (HashMap.add __method__ChurchTest__methodInvokeTest                 METHOD_ChurchTest__methodInvokeTest
+             (HashMap.add __method__ChurchTest__construct                        METHOD_ChurchTest__construct
+             (HashMap.add __method__ChurchTest__testZeroJavalite                 METHOD_ChurchTest__testZeroJavalite
+             (HashMap.add __method__ChurchTest__testNotZeroJavalite              METHOD_ChurchTest__testNotZeroJavalite
+             (HashMap.add __method__ChurchTest__testJavaliteVariableEquivalence  METHOD_ChurchTest__testJavaliteVariableEquivalence
+             (HashMap.add __method__ChurchTest__testJavaliteVariableEquivalence2 METHOD_ChurchTest__testJavaliteVariableEquivalence2
+             (HashMap.empty Method)))))))))).
+
+Definition CLASS_Variable :=
+ (ClassDecl C_Variable (Some CLASS_LambdaTerm)
+            (HashMap.add  __field__Variable__fix T_Bool
+             (HashMap.empty T))
+            (HashMap.add  __method__Variable__cas       METHOD_Variable__cas
+             (HashMap.add __method__Variable__isFree    METHOD_Variable__isFree
+             (HashMap.add __method__Variable__ar        METHOD_Variable__ar
+             (HashMap.add __method__Variable__isAe      METHOD_Variable__isAe
+             (HashMap.add __method__Variable__eval      METHOD_Variable__eval
+             (HashMap.empty Method))))))).
+
+Definition CLASS_Church :=
+ (ClassDecl C_Church CLASS_Object
+            (HashMap.add  __field__Church__x    (T_Class C_Variable)
+             (HashMap.add __field__Church__f    (T_Class C_Variable)
+             (HashMap.add __field__Church__m    (T_Class C_Variable)
+             (HashMap.add __field__Church__n    (T_Class C_Variable)
+             (HashMap.add __field__Church__g    (T_Class C_Variable)
+             (HashMap.add __field__Church__h    (T_Class C_Variable)
+             (HashMap.add __field__Church__u    (T_Class C_Variable)
+             (HashMap.add __field__Church__zero (T_Class C_Abstraction)
+             (HashMap.add __field__Church__one  (T_Class C_Abstraction)
+             (HashMap.add __field__Church__two  (T_Class C_Abstraction)
+             (HashMap.add __field__Church__plus (T_Class C_Abstraction)
+             (HashMap.add __field__Church__succ (T_Class C_Abstraction)
+             (HashMap.add __field__Church__mult (T_Class C_Abstraction)
+             (HashMap.add __field__Church__exp  (T_Class C_Abstraction)
+             (HashMap.empty T)))))))))))))))
+            (HashMap.add  __method__Church__construct METHOD_Church__construct
+             (HashMap.add __method__Church__zero      METHOD_Church__zero
+             (HashMap.add __method__Church__one       METHOD_Church__one
+(*
+             (HashMap.add __method__Church__plus      METHOD_Church__plus
+             (HashMap.add __method__Church__succ      METHOD_Church__succ
+             (HashMap.add __method__Church__mult      METHOD_Church__mult
+             (HashMap.add __method__Church__exp       METHOD_Church__exp
+             (HashMap.add __method__Church__pred      METHOD_Church__pred
+             (HashMap.add __method__Church__minus     METHOD_Church__minus
+*)
+             (HashMap.empty Method))))).
+
+Definition CLASS_SetIfNotZero :=
+ (ClassDecl C_SetIfNotZero CLASS_Object
+            (HashMap.add   __field__SetIfNotZero__x   (T_Class C_Variable)
+             (HashMap.add  __field__SetIfNotZero__y   (T_Class C_Variable)
+             (HashMap.add  __field__SetIfNotZero__bam T_Bool
+             (HashMap.empty T))))
+            (HashMap.add  __method__SetIfNotZero__construct METHOD_SetIfNotZero__construct
+             (HashMap.add __method__SetIfNotZero__eval      METHOD_SetIfNotZero__eval
+             (HashMap.add __method__SetIfNotZero__doEval    METHOD_SetIfNotZero__doEval
+             (HashMap.empty Method))))).
+
+Definition mu_Church : Mu :=
+ (HashMap.add __class__Abstraction  CLASS_Abstraction
+ (HashMap.add __class__Application  CLASS_Application
+ (HashMap.add __class__Church       CLASS_Church
+ (HashMap.add __class__ChurchTest   CLASS_ChurchTest
+ (HashMap.add __class__Function     CLASS_Function
+ (HashMap.add __class__LambdaTerm   CLASS_LambdaTerm
+ (HashMap.add __class__SetIfNotZero CLASS_SetIfNotZero
+ (HashMap.add __class__Variable     CLASS_Variable
+ (HashMap.empty CL))))))))).
+
+Definition ChurchTestProgram : P := (Program mu_Church (EntryPoint C_ChurchTest __method__ChurchTest__construct)).
+
+Definition initialState := inject ChurchTestProgram.
+Definition testNotZeroJavalite := inject_with_state initialState __method__ChurchTest__testNotZeroJavalite.
+Definition mlProgram := (ExprReduces_dec testNotZeroJavalite).
+
+Extraction "javalite.ml" mlProgram.
+
+(* ========================================================================== *)
+(* The Swap program *)
+
+Definition __class__Swap     := (P_of_succ_nat 1).
+Definition __class__SwapTest := (P_of_succ_nat 2).
+
+Definition __field__Swap__a            := (P_of_succ_nat 3).
+Definition __field__Swap__b            := (P_of_succ_nat 4).
+Definition __field__SwapTest__instance := (P_of_succ_nat 5).
+
+Definition __method__Swap__construct   := (P_of_succ_nat 6).
+Definition __method__Swap__swap        := (P_of_succ_nat 7).
+
+Definition __method__SwapTest__construct  := (P_of_succ_nat 8).
+Definition __method__SwapTest__testSwap   := (P_of_succ_nat 9).
+
+Definition __local__Swap__construct__tmp   := (P_of_succ_nat 10).
+Definition __local__SwapTest__construct__v := (P_of_succ_nat 11).
+Definition __local__SwapTest__testSwap__c  := (P_of_succ_nat 12).
+
+Definition C_Swap     := (SomeClass __class__Swap).
+Definition C_SwapTest := (SomeClass __class__SwapTest).
+
+Definition METHOD_Swap__construct :=
+ (AMethod __method__Swap__construct
+          (T_Class C_Swap)
+          nil
+          (SeqExp (FieldAssign This __field__Swap__a (Expr_V (V_Bool false)))
+                  (SeqExp (FieldAssign This __field__Swap__b (Expr_V (V_Bool true)))
+                          (Expr_X (This))))).
+
+Definition METHOD_Swap__swap :=
+ (AMethod __method__Swap__construct
+          (T_Class C_Swap)
+          nil
+          (VarDecExp (VarDec __local__Swap__construct__tmp T_Bool)
+                     (FieldRef (Expr_X This) __field__Swap__b)
+                     (SeqExp (FieldAssign This __field__Swap__b (FieldRef (Expr_X This) __field__Swap__a))
+                             (FieldAssign This __field__Swap__a (Expr_X (SomeId __local__Swap__construct__tmp)))))).
+
+Definition METHOD_SwapTest__construct :=
+ (AMethod __method__SwapTest__construct
+          (T_Class C_SwapTest)
+          nil
+          (VarDecExp (VarDec __local__SwapTest__construct__v (T_Class C_Swap))
+                     (MethodInvocation (NewClass C_Swap) __method__Swap__construct nil)
+                     (SeqExp (FieldAssign This __field__SwapTest__instance (Expr_X (SomeId __local__SwapTest__construct__v)))
+                             (Expr_X This)))).
+
+(*
+(bool testSwap ()
+                (var Swap c := (this $ instance) in
+                     (begin
+                       (c @ swap ())
+                       (if (c $ a)
+                           (if (c $ b)
+                               false
+                               else
+                               true)
+                           else
+                           false))
+                       ))
+*)
+Definition METHOD_SwapTest__testSwap :=
+ (AMethod __method__SwapTest__testSwap
+          T_Bool
+          nil
+          (VarDecExp (VarDec __local__SwapTest__testSwap__c (T_Class C_Swap))
+                     (FieldRef (Expr_X This) __field__SwapTest__instance)
+                     (SeqExp (MethodInvocation (Expr_X (SomeId __local__SwapTest__testSwap__c))
+                                               __method__Swap__swap nil)
+                             (IfExpr (FieldRef (Expr_X (SomeId __local__SwapTest__testSwap__c)) __field__Swap__a)
+                                     (IfExpr (FieldRef (Expr_X (SomeId __local__SwapTest__testSwap__c)) __field__Swap__b)
+                                             (Expr_V (V_Bool false))
+                                             (Expr_V (V_Bool true)))
+                                     (Expr_V (V_Bool false)))))).
+
+Definition CLASS_Swap :=
+ (ClassDecl C_Swap CLASS_Object
+            (HashMap.add   __field__Swap__a T_Bool
+             (HashMap.add  __field__Swap__b T_Bool
+             (HashMap.empty T)))
+            (HashMap.add   __method__Swap__construct METHOD_Swap__construct
+             (HashMap.add  __method__Swap__swap METHOD_Swap__swap
+             (HashMap.empty Method)))).
+
+Definition CLASS_SwapTest :=
+ (ClassDecl C_SwapTest CLASS_Object
+            (HashMap.add  __field__SwapTest__instance (T_Class C_Swap) (HashMap.empty T)))
+            (HashMap.add   __method__SwapTest__construct METHOD_SwapTest__construct
+             (HashMap.add  __method__SwapTest__testSwap METHOD_SwapTest__testSwap
+             (HashMap.empty Method))).
+
+Definition mu_Swap : Mu :=
+ (HashMap.add __class__Swap     CLASS_Swap
+ (HashMap.add __class__SwapTest CLASS_SwapTest
+ (HashMap.empty CL))).
+
+Definition SwapTestProgram : P := (Program mu_Swap (EntryPoint C_SwapTest __method__SwapTest__construct)).
+
+Definition initialState_Swap := inject SwapTestProgram.
+Definition testSwap          := inject_with_state initialState_Swap __method__SwapTest__testSwap.
+Definition mlProgram_Swap    := (ExprReduces_dec testSwap).
+
+Extraction "javalite_swap.ml" mlProgram_Swap.
